,

LCNova.v
@@ -1,477 +1,16 @@
 Require Import Coq.Arith.PeanoNat.
 Require Import Coq.Bool.Bool.
 Require Import Coq.Classes.RelationClasses.
-Require Import Coq.Logic.Classical.
-Require Import Coq.Logic.FunctionalExtensionality.
-Require Import Coq.Logic.PropExtensionality.
 Require Import Coq.Lists.List.
+Require Import Coq.Logic.Classical.
 Require Import Coq.micromega.Lia.
 Require Import Coq.Program.Basics.
 
 Global Create HintDb my_hints.
 
-Module MyUtilities.
-
-  Definition case_eq {A : Type} : forall x : A, forall y : A, forall phi : forall x0 : A, x0 = y -> Type, phi y eq_refl -> forall H : x = y, phi x H :=
-    fun x : A =>
-    fun y : A =>
-    fun phi : forall x0 : A, x0 = y -> Type =>
-    fun phi_y : phi y eq_refl =>
-    fun H : eq x y =>
-    match H as H0 in eq _ y0 return forall phi0 : forall x0 : A, x0 = y0 -> Type, phi0 y0 eq_refl -> phi0 x H0 with
-    | eq_refl =>
-      fun phi0 : forall x0 : A, x0 = x -> Type =>
-      fun phi_y0 : phi0 x eq_refl =>
-      phi_y0
-    end phi phi_y
-  .
-
-  Lemma div_mod_uniqueness :
-    forall a : nat,
-    forall b : nat,
-    forall q : nat,
-    forall r : nat,
-    a = b * q + r ->
-    r < b ->
-    a / b = q /\ a mod b = r.
-  Proof with try (lia || now (firstorder; eauto)).
-    assert (H : forall x : nat, forall y : nat, x > y <-> (exists z : nat, x = S (y + z))).
-    { intros x y; constructor.
-      - intros H.
-        induction H...
-        destruct IHle as [z H0].
-        exists (S z)...
-      - intros H.
-        destruct H as [z H]...
-    }
-    intros a b q r H1 H2.
-    assert (H0 : a = b * (a / b) + (a mod b)) by now apply (Nat.div_mod a b); lia.
-    assert (H3 : 0 <= a mod b < b) by now apply (Nat.mod_bound_pos a b); lia.
-    assert (H4 : ~ q > a / b).
-    { intros H4.
-      enough (H5 : exists z : nat, q = S (a / b + z))...
-      destruct H5 as [z H5].
-      enough (b * q + r >= b * S (a / b) + r)...
-    }
-    assert (H5 : ~ q < a / b).
-    { intros H5.
-      enough (H6 : exists z : nat, a / b = S (q + z))...
-      destruct H6 as [z H6].
-      enough (b * q + a mod b >= b * S (a / b) + a mod b)...
-    }
-    enough (q = a / b)...
-  Qed.
-
-  Definition first_nat : (nat -> bool) -> nat -> nat :=
-    fun p : nat -> bool =>
-    fix first_nat_fix (n : nat) {struct n} : nat :=
-    match n with
-    | 0 => 0
-    | S n' => if p (first_nat_fix n') then first_nat_fix n' else n
-    end
-  .
-
-  Theorem well_ordering_principle : 
-    forall p : nat -> bool,
-    forall n : nat,
-    p n = true ->
-    let m : nat := first_nat p n in
-    p m = true /\ (forall i : nat, p i = true -> i >= m).
-  Proof with eauto. (* This proof has been improved by JunYoung Clare Jang. *)
-    intros p n H3 m.
-    assert (forall x : nat, p x = true -> p (first_nat p x) = true).
-    { induction x...
-      simpl.
-      destruct (p (first_nat p x)) eqn:H0...
-    }
-    split...
-    intros i H4.
-    enough (forall x : nat, first_nat p x <= x).
-    enough (forall x : nat, p (first_nat p x) = true -> (forall y : nat, x < y -> first_nat p x = first_nat p y)).
-    enough (forall x : nat, forall y : nat, p y = true -> first_nat p x <= y)...
-    - intros x y H2.
-      destruct (Compare_dec.le_lt_dec x y).
-      + eapply Nat.le_trans...
-      + replace (first_nat p x) with (first_nat p y)...
-    - intros x H1 y H2.
-      induction H2; simpl.
-      + rewrite H1...
-      + rewrite <- IHle, H1...
-    - induction x...
-      simpl.
-      destruct (p (first_nat p x)) eqn: H0...
-  Qed.
-
-  Fixpoint sum_from_0_to (n : nat) {struct n} : nat :=
-    match n with
-    | 0 => 0
-    | S n' => n + sum_from_0_to n'
-    end
-  .
-
-  Proposition sum_from_0_to_is :
-    forall n : nat,
-    2 * sum_from_0_to n = n * (S n).
-  Proof with lia.
-    induction n; simpl in *...
-  Qed.
-
-  Fixpoint cantor_pairing (n : nat) {struct n} : nat * nat :=
-    match n with
-    | 0 => (0, 0)
-    | S n' =>
-      match cantor_pairing n' with
-      | (0, y) => (S y, 0)
-      | (S x, y) => (x, S y)
-      end
-    end
-  .
-
-  Lemma cantor_pairing_is_surjective :
-    forall x : nat,
-    forall y : nat,
-    (x, y) = cantor_pairing (sum_from_0_to (x + y) + y).
-  Proof with (lia || eauto).
-    enough (forall z : nat, forall y : nat, forall x : nat, z = x + y -> (x, y) = cantor_pairing (sum_from_0_to z + y))...
-    induction z.
-    - intros y x H.
-      assert (H0 : x = 0)...
-      assert (H1 : y = 0)...
-      subst...
-    - induction y.
-      + intros x H.
-        assert (H0 : x = S z)...
-        subst.
-        simpl.
-        destruct (cantor_pairing (z + sum_from_0_to z + 0)) eqn: H0.
-        assert (H1 : (0, z) = cantor_pairing (sum_from_0_to z + z))...
-        rewrite Nat.add_0_r, Nat.add_comm in H0.
-        rewrite H0 in H1.
-        inversion H1; subst...
-      + intros x H.
-        enough (H0 : (S x, y) = cantor_pairing (sum_from_0_to (S z) + y)).
-        { assert (H1 : z + sum_from_0_to z + S y = sum_from_0_to (S z) + y) by now simpl...
-          simpl.
-          rewrite H1, <- H0...
-        }
-        apply (IHy (S x))...
-  Qed.
-
-  Lemma cantor_pairing_is_injective :
-    forall n : nat,
-    forall x : nat,
-    forall y : nat,
-    cantor_pairing n = (x, y) ->
-    n = sum_from_0_to (x + y) + y.
-  Proof with (lia || eauto).
-    induction n; simpl.
-    - intros x y H.
-      inversion H; subst...
-    - intros x y H.
-      destruct (cantor_pairing n) as [x' y'] eqn: H0.
-      destruct x'; (inversion H; subst).
-      + repeat (rewrite Nat.add_0_r).
-        simpl.
-        rewrite (IHn 0 y' eq_refl), Nat.add_0_l...
-      + rewrite (IHn (S x) y' eq_refl).
-        assert (H1 : forall x' : nat, S x' + y' = x' + S y')...
-        repeat (rewrite H1)...
-  Qed.
-
-  Corollary cantor_pairing_is :
-    forall n : nat,
-    forall x : nat,
-    forall y : nat,
-    cantor_pairing n = (x, y) <-> n = sum_from_0_to (x + y) + y.
-  Proof with eauto using cantor_pairing_is_injective, cantor_pairing_is_surjective.
-    split...
-    intros H.
-    subst...
-  Qed.
-
-  Definition S_0 {A : Type} : forall n : nat, S n = 0 -> A :=
-    fun n : nat =>
-    fun H0 : S n = 0 =>
-    let H1 : 0 = S n := @eq_ind nat (S n) (fun x : nat => x = S n) eq_refl 0 H0 in
-    let H2 : False := @eq_ind nat 0 (fun x : nat => if Nat.eqb x 0 then True else False) I (S n) H1 in
-    False_rect A H2
-  .
-
-  Definition S_S : forall n1 : nat, forall n2 : nat, S n1 = S n2 -> n1 = n2 :=
-    fun n1 : nat =>
-    fun n2 : nat =>
-    fun H0 : S n1 = S n2 =>
-    @eq_ind nat (S n1) (fun x : nat => n1 = pred x) eq_refl (S n2) H0
-  .
-
-  Inductive FinSet : nat -> Set :=
-  | FZ : forall n : nat, FinSet (S n) 
-  | FS : forall n : nat, FinSet n -> FinSet (S n)
-  .
-
-  Definition FinSet_case0 {P : FinSet 0 -> Type} : forall i : FinSet 0, P i :=
-    fun i : FinSet 0 =>
-    match i as i0 in FinSet Sn return Sn = 0 -> P i with
-    | FZ n => S_0 n
-    | FS n i' => S_0 n
-    end eq_refl
-  .
-
-  Definition FinSet_caseS {n : nat} {P : FinSet (S n) -> Type} : P (FZ n) -> (forall i' : FinSet n, P (FS n i')) -> (forall i : FinSet (S n), P i) :=
-    fun PZ : P (FZ n) =>
-    fun PS : forall i' : FinSet n, P (FS n i') =>
-    fun i : FinSet (S n) =>
-    match i as i0 in FinSet Sn0 return (match Sn0 as Sn1 return FinSet Sn1 -> Type with 0 => FinSet_case0 | S n0 => fun i1 : FinSet (S n0) => forall P0 : FinSet (S n0) -> Type, P0 (FZ n0) -> (forall i' : FinSet n0, P0 (FS n0 i')) -> P0 i1 end) i0 with
-    | FZ n0 => fun P0 : FinSet (S n0) -> Type => fun PZ0 : P0 (FZ n0) => fun PS0 : forall i' : FinSet n0, P0 (FS n0 i') => PZ0
-    | FS n0 i' => fun P0 : FinSet (S n0) -> Type => fun PZ0 : P0 (FZ n0) => fun PS0 : forall i' : FinSet n0, P0 (FS n0 i') => PS0 i'
-    end P PZ PS
-  .
-
-  Definition FinSet_rectS {P : forall n : nat, FinSet n -> Type} : (forall n : nat, P (S n) (FZ n)) -> (forall n : nat, forall i' : FinSet n, P n i' -> P (S n) (FS n i')) -> (forall n : nat, forall i : FinSet (S n), P (S n) i) :=
-    fun PZ : forall n : nat, P (S n) (FZ n) =>
-    fun PS : forall n : nat, forall i' : FinSet n, P n i' -> P (S n) (FS n i') =>
-    fix FinSet_rectS_fix (n : nat) (i : FinSet (S n)) {struct i} : P (S n) i :=
-    match i as i0 in FinSet Sn0 return P Sn0 i0 with
-    | FZ n0 => PZ n0
-    | FS n0 i' =>
-      match n0 as n1 return forall i0' : FinSet n1, P (S n1) (FS n1 i0') with
-      | 0 => fun i0' : FinSet 0 => @FinSet_case0 (fun i1 : FinSet 0 => P 1 (FS 0 i1)) i0'
-      | S n0' => fun i0' : FinSet (S n0') => PS (S n0') i0' (FinSet_rectS_fix n0' i0')
-      end i'
-    end
-  .
-
-
-  Lemma forallb_true_iff {A : Type} {p : A -> bool} (xs : list A) :
-    forallb p xs = true <-> forall x : A, In x xs -> p x = true.
-  Proof with try now firstorder.
-    induction xs; simpl...
-    rewrite andb_true_iff.
-    split...
-    intros H0 x H1.
-    destruct H0; destruct H1...
-    rewrite H1 in H...
-  Qed.
-
-  Definition fold_right_max_0 : list nat -> nat :=
-    fold_right max 0
-  .
-
-  Lemma fold_right_max_0_in :
-    forall ns : list nat,
-    forall n : nat,
-    In n ns ->
-    fold_right_max_0 ns >= n.
-  Proof with (lia || eauto).
-    unfold fold_right_max_0.
-    induction ns as [| n' ns]; simpl...
-    intros n H.
-    destruct H...
-    enough (fold_right max 0 ns >= n)...
-  Qed.
-
-  Lemma fold_right_max_0_app :
-    forall ns1 : list nat,
-    forall ns2 : list nat,
-    fold_right_max_0 (ns1 ++ ns2) = max (fold_right_max_0 ns1) (fold_right_max_0 ns2).
-  Proof with (lia || eauto).
-    unfold fold_right_max_0.
-    induction ns1 as [| n1 ns1]; simpl... 
-    intros n.
-    rewrite IHns1...
-  Qed.
-
-  Lemma property1_of_fold_right_max_0 (Phi : nat -> Prop) (Phi_dec : forall i : nat, {Phi i} + {~ Phi i}) :
-    forall ns : list nat,
-    (forall i : nat, Phi i -> In i ns) ->
-    forall n : nat,
-    Phi n ->
-    fold_right max 0 ns >= n.
-  Proof with (lia || eauto).
-    induction ns; simpl.
-    - intros H n H0.
-      contradiction (H n).
-    - intros H n H0.
-      destruct (Compare_dec.le_lt_dec n a)...
-      enough (fold_right max 0 ns >= n)...
-      destruct (Phi_dec n).
-      + destruct (H n p)...
-        enough (forall ks : list nat, forall k : nat, In k ks -> fold_right max 0 ks >= k) by firstorder.
-        induction ks; simpl...
-        intros k H2.
-        destruct H2...
-        enough (fold_right Init.Nat.max 0 ks >= k)...
-      + apply IHns...
-        intros.
-        destruct (H i H1)...
-        subst.
-        contradiction.
-  Qed.
-
-  Lemma property2_of_fold_right_max_0 :
-    forall ns : list nat,
-    forall n : nat,
-    fold_right max 0 ns > n <-> (exists i : nat, In i ns /\ i > n).
-  Proof with (lia || eauto).
-    induction ns; simpl.
-    - split...
-      now firstorder.
-    - intros n.
-      destruct (Compare_dec.le_lt_dec a (fold_right Init.Nat.max 0 ns)); split...
-      + intros H.
-        assert (H0 : fold_right Init.Nat.max 0 ns > n)...
-        destruct (proj1 (IHns n) H0) as [i].
-        now firstorder.
-      + intros H.
-        destruct H as [i].
-        destruct H.
-        destruct H.
-        * subst...
-        * enough (fold_right max 0 ns > n)...
-          apply IHns...
-      + intros H.
-        exists a...
-      + intros H.
-        destruct H as [i].
-        destruct H.
-        destruct H.
-        * subst...
-        * enough (fold_right Init.Nat.max 0 ns > n)...
-          apply IHns...
-  Qed.
-
-  Lemma property3_of_fold_right_max_0 :
-    forall ns1 : list nat,
-    forall ns2 : list nat,
-    fold_right max 0 (ns1 ++ ns2) = max (fold_right max 0 ns1) (fold_right max 0 ns2).
-  Proof.
-    apply fold_right_max_0_app.
-  Qed.
-
-  Lemma property4_of_fold_right_max_0 :
-    forall ns : list nat,
-    forall n : nat,
-    In n ns ->
-    fold_right max 0 ns >= n.
-  Proof with (lia || eauto).
-    induction ns; simpl...
-    intros n H.
-    destruct H...
-    enough (fold_right max 0 ns >= n)...
-  Qed.
-
-  Lemma property5_of_fold_right_max_0 :
-    forall ns1 : list nat,
-    forall ns2 : list nat,
-    (forall n : nat, In n ns1 -> In n ns2) ->
-    fold_right max 0 ns1 <= fold_right max 0 ns2.
-  Proof with (lia || eauto).
-    induction ns1; simpl...
-    intros ns2 H.
-    destruct (Compare_dec.le_lt_dec a (fold_right max 0 ns1)).
-    - enough (fold_right max 0 ns1 <= fold_right max 0 ns2)...
-    - enough (a <= fold_right max 0 ns2)...
-      apply property4_of_fold_right_max_0...
-  Qed.
-
-  Lemma fold_right_max_0_ext :
-    forall ns1 : list nat,
-    forall ns2 : list nat,
-    (forall n : nat, In n ns1 <-> In n ns2) ->
-    fold_right max 0 ns1 = fold_right max 0 ns2.
-  Proof with try now firstorder.
-    intros.
-    enough (fold_right max 0 ns1 <= fold_right max 0 ns2 /\ fold_right max 0 ns2 <= fold_right max 0 ns1) by lia.
-    split; apply property5_of_fold_right_max_0...
-  Qed.
-
-End MyUtilities.
-
 Module MyStructures.
 
-  Class isPoset (A : Type) : Type :=
-    { leProp : A -> A -> Prop
-    ; Poset_requiresPreOrder :> PreOrder leProp
-    ; Poset_requiresPartialOrder :> PartialOrder (@eq A) leProp
-    }
-  .
-
-  Global Hint Resolve Poset_requiresPreOrder : my_hints.
-
-  Global Hint Resolve Poset_requiresPartialOrder : my_hints.
-
-  Global Notation "x =< y" := (leProp x y) (at level 70, no associativity) : type_scope.
-
-  Lemma Poset_refl {A : Type} `{A_isPoset : isPoset A} :
-    forall x : A,
-    x =< x.
-  Proof.
-    apply Poset_requiresPreOrder.
-  Qed.
-
-  Global Hint Resolve Poset_refl : my_hints.
-
-  Lemma Poset_refl1 {A : Type} `{A_isPoset : isPoset A} :
-    forall x1 : A,
-    forall x2 : A,
-    x1 = x2 ->
-    x1 =< x2.
-  Proof.
-    apply Poset_requiresPartialOrder.
-  Qed.
-
-  Global Hint Resolve Poset_refl1 : my_hints.
-
-  Lemma Poset_refl2 {A : Type} `{A_isPoset : isPoset A} :
-    forall x1 : A,
-    forall x2 : A,
-    x1 = x2 ->
-    x2 =< x1.
-  Proof.
-    apply Poset_requiresPartialOrder.
-  Qed.
-
-  Global Hint Resolve Poset_refl2 : my_hints.
-
-  Lemma Poset_asym {A : Type} `{A_isPoset : isPoset A} :
-    forall x1 : A,
-    forall x2 : A,
-    x1 =< x2 ->
-    x2 =< x1 ->
-    x1 = x2.
-  Proof.
-    intros x1 x2 H H0.
-    apply Poset_requiresPartialOrder.
-    split; [apply H | apply H0].
-  Qed.
-
-  Global Hint Resolve Poset_asym : my_hints.
-
-  Lemma Poset_trans {A : Type} `{A_isPoset : isPoset A} :
-    forall x1 : A,
-    forall x2 : A,
-    forall x3 : A,
-    x1 =< x2 ->
-    x2 =< x3 ->
-    x1 =< x3.
-  Proof.
-    apply Poset_requiresPreOrder.
-  Qed.
-
-  Global Hint Resolve Poset_trans : my_hints.
-
-  Global Program Instance nat_isPoset : isPoset nat :=
-    { leProp := le
-    }
-  .
-
-End MyStructures.
-
-Module MyEnsemble.
-
   Import ListNotations.
-
-  Import MyStructures.
 
   Definition ensemble : Type -> Type :=
     fun A : Type =>
@@ -499,32 +38,6 @@ Module MyEnsemble.
   Global Hint Unfold isSubsetOf : my_hints.
 
   Global Notation "xs1 '\subseteq' xs2" := (isSubsetOf xs1 xs2) (at level 70, no associativity) : type_scope.
-
-  Global Program Instance ensemble_isPoset {A : Type} : isPoset (ensemble A) :=
-    { leProp := isSubsetOf
-    }
-  .
-
-  Next Obligation with eauto with *.
-    split...
-  Qed.
-
-  Next Obligation with eauto with *.
-    intros xs1 xs2.
-    split.
-    - repeat red.
-      split.
-      + subst...
-      + red.
-        subst...
-    - intros [H H0].
-      apply functional_extensionality.
-      intros x.
-      apply propositional_extensionality.
-      split.
-      + apply (H x).
-      + apply (H0 x).
-  Qed.
 
   Inductive finite {A : Type} : list A -> ensemble A :=
   | in_finite {x : A} :
@@ -650,27 +163,218 @@ Module MyEnsemble.
 
   Global Hint Unfold nonempty : my_hints.
 
-End MyEnsemble.
+  Class isSetoid (A : Type) : Type :=
+    { eqProp : A -> A -> Prop
+    ; Setoid_requiresEquivalence :> Equivalence eqProp
+    }
+  .
 
-Module GeneralTopology.
+  Global Notation "x == y" := (eqProp x y) (at level 70, no associativity) : type_scope.
 
-  Import ListNotations.
+  Lemma Setoid_refl {A : Type} `{A_isSetoid : isSetoid A} :
+    forall x1 : A,
+    x1 == x1.
+  Proof.
+    apply Setoid_requiresEquivalence.
+  Qed.
 
-  Import MyStructures.
+  Global Hint Resolve Setoid_refl : my_hints.
 
-  Import MyEnsemble.
+  Lemma Setoid_sym {A : Type} `{A_isSetoid : isSetoid A} :
+    forall x1 : A,
+    forall x2 : A,
+    x1 == x2 ->
+    x2 == x1.
+  Proof.
+    apply Setoid_requiresEquivalence.
+  Qed.
 
-  Class isTopologicalSpace (X : Type) : Type :=
-    { isOpen : ensemble X -> Prop
+  Global Hint Resolve Setoid_sym : my_hints.
+
+  Lemma Setoid_trans {A : Type} `{A_isSetoid : isSetoid A} :
+    forall x1 : A,
+    forall x2 : A,
+    forall x3 : A,
+    x1 == x2 ->
+    x2 == x3 ->
+    x1 == x3.
+  Proof.
+    apply Setoid_requiresEquivalence.
+  Qed.
+
+  Global Hint Resolve Setoid_trans : my_hints.
+
+  Definition preservesSetoid {A : Type} {B : Type} `{A_isSetoid : isSetoid A} `{B_isSetoid : isSetoid B} : (A -> B) -> Prop :=
+    fun f : A -> B =>
+    forall x1 : A,
+    forall x2 : A,
+    x1 == x2 ->
+    f x1 == f x2
+  .
+
+  Global Hint Unfold preservesSetoid : my_hints.
+
+  Global Program Instance arrow_isSetoid {A : Type} {B : Type} (B_requiresSetoid : isSetoid B) : isSetoid (A -> B) :=
+    { eqProp :=
+      fun f1 : A -> B =>
+      fun f2 : A -> B =>
+      forall x : A,
+      f1 x == f2 x
+    }
+  .
+
+  Next Obligation with eauto with *.
+    split...
+  Qed.
+
+  Global Program Instance ensemble_isSetoid {A : Type} : isSetoid (ensemble A) :=
+    { eqProp :=
+      fun X1 : ensemble A =>
+      fun X2 : ensemble A =>
+      forall x : A,
+      member x X1 <-> member x X2
+    }
+  .
+
+  Next Obligation with firstorder with my_hints.
+    split...
+  Qed.
+
+  Class isPoset (A : Type) : Type :=
+    { leProp : A -> A -> Prop
+    ; Poset_requiresSetoid :> isSetoid A
+    ; Poset_requiresPreOrder :> PreOrder leProp
+    ; Poset_requiresPartialOrder :> PartialOrder eqProp leProp
+    }
+  .
+
+  Global Notation "x =< y" := (leProp x y) (at level 70, no associativity) : type_scope.
+
+  Lemma Poset_refl {A : Type} `{A_isPoset : isPoset A} :
+    forall x1 : A,
+    x1 =< x1.
+  Proof.
+    apply Poset_requiresPreOrder.
+  Qed.
+
+  Global Hint Resolve Poset_refl : my_hints.
+
+  Lemma Poset_refl1 {A : Type} `{A_isPoset : isPoset A} :
+    forall x1 : A,
+    forall x2 : A,
+    x1 == x2 ->
+    x1 =< x2.
+  Proof.
+    apply Poset_requiresPartialOrder.
+  Qed.
+
+  Global Hint Resolve Poset_refl1 : my_hints.
+
+  Lemma Poset_refl2 {A : Type} `{A_isPoset : isPoset A} :
+    forall x1 : A,
+    forall x2 : A,
+    x1 == x2 ->
+    x2 =< x1.
+  Proof.
+    apply Poset_requiresPartialOrder.
+  Qed.
+
+  Global Hint Resolve Poset_refl2 : my_hints.
+
+  Lemma Poset_asym {A : Type} `{A_isPoset : isPoset A} :
+    forall x1 : A,
+    forall x2 : A,
+    x1 =< x2 ->
+    x2 =< x1 ->
+    x1 == x2.
+  Proof.
+    intros x1 x2 H H0.
+    apply Poset_requiresPartialOrder.
+    split.
+    - apply H.
+    - apply H0.
+  Qed.
+
+  Global Hint Resolve Poset_asym : my_hints.
+
+  Lemma Poset_trans {A : Type} `{A_isPoset : isPoset A} :
+    forall x1 : A,
+    forall x2 : A,
+    forall x3 : A,
+    x1 =< x2 ->
+    x2 =< x3 ->
+    x1 =< x3.
+  Proof.
+    apply Poset_requiresPreOrder.
+  Qed.
+
+  Global Hint Resolve Poset_trans : my_hints.
+
+  Definition isMonotonicMap {A : Type} {B : Type} `{A_isPoset : isPoset A} `{B_isPoset : isPoset B} : (A -> B) -> Prop :=
+    fun f : A -> B =>
+    forall x1 : A,
+    forall x2 : A,
+    x1 =< x2 ->
+    f x1 =< f x2
+  .
+
+  Global Hint Unfold isMonotonicMap : my_hints.
+
+  Lemma MonotonicMap_preservesSetoid {A : Type} {B : Type} `{A_isPoset : isPoset A} `{B_isPoset : isPoset B} :
+    forall f : A -> B,
+    isMonotonicMap f ->
+    preservesSetoid f.
+  Proof with eauto with *.
+    unfold isMonotonicMap, preservesSetoid.
+    intros f H x1 x2 H0.
+    apply Poset_asym...
+  Qed.
+
+  Global Hint Unfold MonotonicMap_preservesSetoid : my_hints.
+
+  Definition isSupremum {A : Type} `{A_isPoset : isPoset A} : A -> ensemble A -> Prop :=
+    fun sup_X : A =>
+    fun X : ensemble A =>
+    forall a : A,
+    sup_X =< a <-> (forall x : A, member x X -> x =< a)
+  .
+
+  Global Hint Unfold isSupremum : my_hints.
+
+  Definition isInfimum {A : Type} `{A_isPoset : isPoset A} : A -> ensemble A -> Prop :=
+    fun inf_X : A =>
+    fun X : ensemble A =>
+    forall a : A,
+    a =< inf_X <-> (forall x : A, member x X -> a =< x)
+  .
+
+  Global Hint Unfold isInfimum : my_hints.
+
+  Global Program Instance ensemble_isPoset {A : Type} : isPoset (ensemble A) :=
+    { leProp := isSubsetOf
+    ; Poset_requiresSetoid := ensemble_isSetoid
+    }
+  .
+
+  Next Obligation with eauto with *.
+    split...
+  Qed.
+
+  Next Obligation with firstorder.
+    split...
+  Qed.
+
+  Class isTopologicalSpace (A : Type) : Type :=
+    { isOpen : ensemble A -> Prop
     ; open_for_full :
       isOpen full
     ; open_for_unions :
-      forall xss : ensemble (ensemble X),
-      (forall xs : ensemble X, member xs xss -> isOpen xs) ->
+      forall xss : ensemble (ensemble A),
+      (forall xs : ensemble A, member xs xss -> isOpen xs) ->
       isOpen (unions xss)
     ; open_for_intersection :
-      forall xs1 : ensemble X,
-      forall xs2 : ensemble X,
+      forall xs1 : ensemble A,
+      forall xs2 : ensemble A,
       isOpen xs1 ->
       isOpen xs2 ->
       isOpen (intersection xs1 xs2)
@@ -683,35 +387,29 @@ Module GeneralTopology.
 
   Global Hint Resolve open_for_intersection : my_hints.
 
-  Definition isContinuousMap {X : Type} {Y : Type} `{X_isTopologicalSpace : isTopologicalSpace X} `{Y_isTopologicalSpace : isTopologicalSpace Y} : (X -> Y) -> Prop :=
-    fun f : X -> Y =>
-    forall ys : ensemble Y,
+  Definition isClosed {A : Type} `{A_isTopologicalSpace : isTopologicalSpace A} : ensemble A -> Prop :=
+    fun X : ensemble A =>
+    isOpen (fun x : A => ~ member x X)
+  .
+
+  Global Hint Unfold isClosed : my_hints.
+
+  Definition isContinuousMap {A : Type} {B : Type} `{A_isTopologicalSpace : isTopologicalSpace A} `{B_isTopologicalSpace : isTopologicalSpace B} : (A -> B) -> Prop :=
+    fun f : A -> B =>
+    forall ys : ensemble B,
     isOpen ys ->
     isOpen (preimage f ys)
   .
 
   Global Hint Unfold isContinuousMap : my_hints.
 
-End GeneralTopology.
+End MyStructures.
 
 Module DomainTheory.
 
   Import ListNotations.
 
   Import MyStructures.
-
-  Import MyEnsemble.
-
-  Import GeneralTopology.
-
-  Definition isSupremum {D : Type} `{D_isPoset : isPoset D} : D -> ensemble D -> Prop :=
-    fun sup_X : D =>
-    fun X : ensemble D =>
-    forall d : D,
-    sup_X =< d <-> (forall x : D, member x X -> x =< d)
-  .
-
-  Global Hint Unfold isSupremum : my_hints.
 
   Lemma isSupremum_upperbound {D : Type} `{D_isPoset : isPoset D} :
     forall sup_X : D,
@@ -750,7 +448,7 @@ Module DomainTheory.
     forall sup_X1 : D,
     isSupremum sup_X1 X1 ->
     forall sup_X2 : D,
-    isSupremum sup_X2 X2 <-> sup_X1 = sup_X2.
+    isSupremum sup_X2 X2 <-> sup_X1 == sup_X2.
   Proof with eauto with *.
     intros X1 X2 H sup_X1 H0 sup_X2.
     assert (claim1 := fun x : D => fun H1 : member x X1 => proj1 (H x) H1).
@@ -773,7 +471,7 @@ Module DomainTheory.
     forall sup1 : D,
     isSupremum sup1 X ->
     forall sup2 : D,
-    isSupremum sup2 X <-> sup1 = sup2.
+    isSupremum sup2 X <-> sup1 == sup2.
   Proof with eauto with *.
     intros X sup1 H sup2...
   Qed.
@@ -835,15 +533,44 @@ Module DomainTheory.
         apply H3...
   Qed.
 
+  Global Hint Resolve isSupremum_unions_Xs_iff_isSupremum_image_sup_Xs : my_hints.
+
   Class isCompleteLattice (D : Type) : Type :=
     { CompleteLattice_requiresPoset :> isPoset D
-    ; supremum_always_exists :
+    ; supremum_always_exists_in_CompleteLattice :
       forall X : ensemble D,
       {sup_X : D | isSupremum sup_X X}
     }
   .
 
-  Global Hint Resolve supremum_always_exists : my_hints.
+  Global Hint Resolve CompleteLattice_requiresPoset : my_hints.
+
+  Lemma compute_Infimum_in_CompleteLattice {D : Type} `{D_isCompleteLattice : isCompleteLattice D} :
+    forall X : ensemble D,
+    forall inf_X : D,
+    isSupremum inf_X (fun d : D => forall x : D, member x X -> d =< x) ->
+    isInfimum inf_X X.
+  Proof with eauto with *.
+    intros X inf_X H d.
+    split.
+    - intros H0 x H1.
+      transitivity inf_X...
+      apply H...
+    - intros H0.
+      apply H...
+  Qed.
+
+  Global Hint Resolve compute_Infimum_in_CompleteLattice : my_hints.
+
+  Definition infimum_always_exists_in_CompleteLattice {D : Type} `{D_isCompleteLattice : isCompleteLattice D} :
+    forall X : ensemble D,
+    {inf_X : D | isInfimum inf_X X}.
+  Proof.
+    intros X.
+    destruct (supremum_always_exists_in_CompleteLattice (fun d : D => forall x : D, member x X -> d =< x)) as [inf_X H].
+    exists inf_X.
+    apply compute_Infimum_in_CompleteLattice, H.
+  Defined.
 
   Lemma unions_isSupremum {A : Type} :
     forall Xs : ensemble (ensemble A),
@@ -862,11 +589,458 @@ Module DomainTheory.
 
   Global Instance ensemble_isCompleteLattice {A : Type} : isCompleteLattice (ensemble A) :=
     { CompleteLattice_requiresPoset := ensemble_isPoset
-    ; supremum_always_exists :=
+    ; supremum_always_exists_in_CompleteLattice :=
       fun Xs : ensemble (ensemble A) =>
-      exist _ (unions Xs) (unions_isSupremum Xs)
+      exist (fun unions_Xs : ensemble A => isSupremum unions_Xs Xs) (unions Xs) (unions_isSupremum Xs)
     }
   .
+
+  Definition monotonic_map {D : Type} {D' : Type} : isPoset D -> isPoset D' -> Type :=
+    fun D_requiresPoset : isPoset D =>
+    fun D'_requiresPoset : isPoset D' =>
+    {f : D -> D' | isMonotonicMap f}
+  .
+
+  Global Program Instance MonotonicMap_isSetoid {D : Type} {D' : Type} (D_requiresPoset : isPoset D) (D'_requiresPoset : isPoset D') : isSetoid (monotonic_map D_requiresPoset D'_requiresPoset) :=
+    { eqProp :=
+      fun f1 : monotonic_map D_requiresPoset D'_requiresPoset =>
+      fun f2 : monotonic_map D_requiresPoset D'_requiresPoset =>
+      forall x : D,
+      proj1_sig f1 x == proj1_sig f2 x
+    }
+  .
+
+  Next Obligation with eauto with *.
+    split...
+  Qed.
+
+  Global Program Instance MonotonicMap_can_be_pointwise_partially_ordered {D : Type} {D' : Type} (D_requiresPoset : isPoset D) (D'_requiresPoset : isPoset D') : isPoset (monotonic_map D_requiresPoset D'_requiresPoset) :=
+    { leProp :=
+      fun f1 : monotonic_map D_requiresPoset D'_requiresPoset =>
+      fun f2 : monotonic_map D_requiresPoset D'_requiresPoset =>
+      forall x : D,
+      proj1_sig f1 x =< proj1_sig f2 x
+    ; Poset_requiresSetoid := MonotonicMap_isSetoid D_requiresPoset D'_requiresPoset
+    }
+  .
+
+  Next Obligation with eauto with *.
+    split...
+  Qed.
+
+  Next Obligation with firstorder with my_hints.
+    split...
+  Qed.
+
+  Definition supOfMonotonicMaps {D : Type} {D' : Type} `{D_isCompleteLattice : isCompleteLattice D} `{D'_isCompleteLattice : isCompleteLattice D'} : ensemble (monotonic_map (@CompleteLattice_requiresPoset D D_isCompleteLattice) (@CompleteLattice_requiresPoset D' D'_isCompleteLattice)) -> D -> D' :=
+    fun fs : ensemble (monotonic_map (@CompleteLattice_requiresPoset D D_isCompleteLattice) (@CompleteLattice_requiresPoset D' D'_isCompleteLattice)) =>
+    fun x : D =>
+    proj1_sig (supremum_always_exists_in_CompleteLattice (image (fun f_i : monotonic_map (@CompleteLattice_requiresPoset D D_isCompleteLattice) (@CompleteLattice_requiresPoset D' D'_isCompleteLattice) => proj1_sig f_i x) fs))
+  .
+
+  Lemma supOfMonotonicMaps_isMonotonic {D : Type} {D' : Type} `{D_isCompleteLattice : isCompleteLattice D} `{D'_isCompleteLattice : isCompleteLattice D'} :
+    forall fs : ensemble (monotonic_map (@CompleteLattice_requiresPoset D D_isCompleteLattice) (@CompleteLattice_requiresPoset D' D'_isCompleteLattice)),
+    isMonotonicMap (supOfMonotonicMaps fs).
+  Proof with eauto with *.
+    intros fs x1 x2 H.
+    unfold supOfMonotonicMaps.
+    destruct (supremum_always_exists_in_CompleteLattice (image (fun f_i : (monotonic_map (@CompleteLattice_requiresPoset D D_isCompleteLattice) (@CompleteLattice_requiresPoset D' D'_isCompleteLattice)) => proj1_sig f_i x1) fs)) as [sup1 H0].
+    destruct (supremum_always_exists_in_CompleteLattice (image (fun f_i : (monotonic_map (@CompleteLattice_requiresPoset D D_isCompleteLattice) (@CompleteLattice_requiresPoset D' D'_isCompleteLattice)) => proj1_sig f_i x2) fs)) as [sup2 H1].
+    simpl.
+    apply H0.
+    intros x H2.
+    inversion H2; subst.
+    rename x0 into f_i.
+    transitivity (proj1_sig f_i x2).
+    - apply (proj2_sig f_i)...
+    - apply H1...
+      apply (in_image (fun f_i' : monotonic_map (@CompleteLattice_requiresPoset D D_isCompleteLattice) (@CompleteLattice_requiresPoset D' D'_isCompleteLattice) => proj1_sig f_i' x2))...
+  Qed.
+
+  Lemma supOfMonotonicMaps_isSupremum {D : Type} {D' : Type} `{D_isCompleteLattice : isCompleteLattice D} `{D'_isCompleteLattice : isCompleteLattice D'} :
+    forall fs : ensemble (monotonic_map (@CompleteLattice_requiresPoset D D_isCompleteLattice) (@CompleteLattice_requiresPoset D' D'_isCompleteLattice)),
+    isSupremum (exist isMonotonicMap (supOfMonotonicMaps fs) (supOfMonotonicMaps_isMonotonic fs)) fs.
+  Proof with eauto with *.
+    intros fs f.
+    split.
+    - intros H0 f' H1.
+      transitivity (exist isMonotonicMap (supOfMonotonicMaps fs) (supOfMonotonicMaps_isMonotonic fs))...
+      intros x.
+      simpl.
+      apply (proj2_sig (supremum_always_exists_in_CompleteLattice (image (fun f_i : monotonic_map (@CompleteLattice_requiresPoset D D_isCompleteLattice) (@CompleteLattice_requiresPoset D' D'_isCompleteLattice) => proj1_sig f_i x) fs)))...
+      apply (in_image (fun f_i' : monotonic_map (@CompleteLattice_requiresPoset D D_isCompleteLattice) (@CompleteLattice_requiresPoset D' D'_isCompleteLattice) => proj1_sig f_i' x))...
+    - intros H x.
+      simpl.
+      apply (proj2_sig (supremum_always_exists_in_CompleteLattice (image (fun f_i : monotonic_map (@CompleteLattice_requiresPoset D D_isCompleteLattice) (@CompleteLattice_requiresPoset D' D'_isCompleteLattice) => proj1_sig f_i x) fs)))...
+      intros f' H0.
+      inversion H0; subst.
+      rename x0 into f'.
+      apply (H f' H1 x).
+  Qed.
+
+  Global Instance MonotonicMaps_on_CompleteLattice_constitute_CompleteLattice {D : Type} {D' : Type} (D_requiresCompleteLattice : isCompleteLattice D) (D'_requiresCompleteLattice : isCompleteLattice D') : isCompleteLattice (monotonic_map (@CompleteLattice_requiresPoset D D_requiresCompleteLattice) (@CompleteLattice_requiresPoset D' D'_requiresCompleteLattice)) :=
+    { CompleteLattice_requiresPoset := MonotonicMap_can_be_pointwise_partially_ordered (@CompleteLattice_requiresPoset D D_requiresCompleteLattice) (@CompleteLattice_requiresPoset D' D'_requiresCompleteLattice)
+    ; supremum_always_exists_in_CompleteLattice :=
+      fun fs : ensemble (monotonic_map (@CompleteLattice_requiresPoset D D_requiresCompleteLattice) (@CompleteLattice_requiresPoset D' D'_requiresCompleteLattice)) =>
+      exist _ (exist _ (supOfMonotonicMaps fs) (supOfMonotonicMaps_isMonotonic fs)) (supOfMonotonicMaps_isSupremum fs)
+    }
+  .
+
+  Definition fixed_points {D : Type} `{D_isPoset : isPoset D} : (D -> D) -> ensemble D :=
+    fun f : D -> D =>
+    fun fix_f : D =>
+    fix_f == f fix_f
+  .
+
+  Global Hint Unfold fixed_points : my_hints.
+
+  Definition isLeastFixedPoint {D : Type} `{D_isPoset : isPoset D} : D -> (D -> D) -> Prop :=
+    fun lfp : D =>
+    fun f : D -> D =>
+    member lfp (fixed_points f) /\ (forall fix_f : D, member fix_f (fixed_points f) -> lfp =< fix_f)
+  .
+
+  Global Hint Unfold isLeastFixedPoint : my_hints.
+
+  Lemma LeastFixedPointOfPoset {D : Type} `{D_isPoset : isPoset D} :
+    forall f : D -> D,
+    isMonotonicMap f ->
+    forall lfp : D,
+    isInfimum lfp (fun x : D => f x =< x) ->
+    isLeastFixedPoint lfp f.
+  Proof with eauto with *.
+    intros f H lfp H0.
+    split.
+    - assert (H1 : f lfp =< lfp).
+      { apply H0.
+        intros x H1.
+        transitivity (f x)...
+        apply H...
+        transitivity (f x)...
+        apply H0...
+      }
+      apply Poset_asym.
+      + apply H0...
+      + apply H1.
+    - intros fix_f H1.
+      apply H0...
+  Qed.
+
+  Lemma LeastFixedPointOfCompleteLattice {D : Type} `{D_isCompleteLattice : isCompleteLattice D} :
+    forall f : D -> D,
+    isMonotonicMap f ->
+    exists lfp : D, isInfimum lfp (fun x : D => f x =< x) /\ isLeastFixedPoint lfp f.
+  Proof with eauto with *.
+    intros f H.
+    destruct (infimum_always_exists_in_CompleteLattice (fun x : D => f x =< x)) as [lfp H0].
+    exists lfp.
+    split...
+    apply LeastFixedPointOfPoset...
+  Qed.
+
+  Definition isGreatestFixedPoint {D : Type} `{D_isPoset : isPoset D} : D -> (D -> D) -> Prop :=
+    fun gfp : D =>
+    fun f : D -> D =>
+    member gfp (fixed_points f) /\ (forall fix_f : D, member fix_f (fixed_points f) -> fix_f =< gfp)
+  .
+
+  Global Hint Unfold isGreatestFixedPoint : my_hints.
+
+  Lemma GreatestFixedPointOfPoset {D : Type} `{D_isPoset : isPoset D} :
+    forall f : D -> D,
+    isMonotonicMap f ->
+    forall gfp : D,
+    isSupremum gfp (fun x : D => x =< f x) ->
+    isGreatestFixedPoint gfp f.
+  Proof with eauto with *.
+    intros f H gfp H0.
+    split.
+    - assert (H1 : gfp =< f gfp).
+      { apply H0.
+        intros x H1.
+        transitivity (f x)...
+      }
+      apply Poset_asym.
+      + apply H1.
+      + apply H0...
+    - intros fix_f H1.
+      apply H0...
+  Qed.
+
+  Lemma GreatestFixedPointOfCompleteLattice {D : Type} `{D_isCompleteLattice : isCompleteLattice D} :
+    forall f : D -> D,
+    isMonotonicMap f ->
+    exists gfp : D, isSupremum gfp (fun x : D => x =< f x) /\ isGreatestFixedPoint gfp f.
+  Proof with eauto with *.
+    intros f H.
+    destruct (supremum_always_exists_in_CompleteLattice (fun x : D => x =< f x)) as [gfp H0].
+    exists gfp.
+    split...
+    apply GreatestFixedPointOfPoset...
+  Qed.
+
+  Definition nu {D : Type} `{D_isCompleteLattice : isCompleteLattice D} : forall f : monotonic_map (@CompleteLattice_requiresPoset D D_isCompleteLattice) (@CompleteLattice_requiresPoset D D_isCompleteLattice), {gfp : D | isGreatestFixedPoint gfp (proj1_sig f)} :=
+    fun f : monotonic_map (@CompleteLattice_requiresPoset D D_isCompleteLattice) (@CompleteLattice_requiresPoset D D_isCompleteLattice) =>
+    match supremum_always_exists_in_CompleteLattice (fun x : D => x =< proj1_sig f x) with
+    | exist _ gfp H => exist _ gfp (GreatestFixedPointOfPoset (proj1_sig f) (proj2_sig f) gfp H)
+    end
+  .
+
+  Definition or_plus {D : Type} `{D_isCompleteLattice : isCompleteLattice D} : D -> D -> D :=
+    fun x1 : D =>
+    fun x2 : D =>
+    proj1_sig (supremum_always_exists_in_CompleteLattice (finite [x1; x2]))
+  .
+
+  Lemma le_or_plus {D : Type} `{D_isCompleteLattice : isCompleteLattice D} :
+    forall x1 : D,
+    forall x2 : D,
+    x1 =< or_plus x1 x2 /\ x2 =< or_plus x1 x2.
+  Proof with eauto with *.
+    intros x1 x2.
+    assert (H : isSupremum (or_plus x1 x2) (finite [x1; x2])) by apply (proj2_sig (supremum_always_exists_in_CompleteLattice (finite [x1; x2]))).
+    split...
+  Qed.
+
+  Lemma le_or_plus1 {D : Type} `{D_isCompleteLattice : isCompleteLattice D} :
+    forall x1 : D,
+    forall x2 : D,
+    x1 =< or_plus x1 x2.
+  Proof.
+    apply le_or_plus.
+  Defined.
+
+  Global Hint Resolve le_or_plus1 : my_hints.
+
+  Lemma le_or_plus2 {D : Type} `{D_isCompleteLattice : isCompleteLattice D} :
+    forall x1 : D,
+    forall x2 : D,
+    x2 =< or_plus x1 x2.
+  Proof.
+    apply le_or_plus.
+  Defined.
+
+  Global Hint Resolve le_or_plus2 : my_hints.
+
+  Lemma or_plus_le_iff {D : Type} `{D_isCompleteLattice : isCompleteLattice D} :
+    forall x1 : D,
+    forall x2 : D,
+    forall d : D,
+    or_plus x1 x2 =< d <-> (x1 =< d /\ x2 =< d).
+  Proof with eauto with *.
+    intros x1 x2 d.
+    assert (H : isSupremum (or_plus x1 x2) (finite [x1; x2])) by apply (proj2_sig (supremum_always_exists_in_CompleteLattice (finite [x1; x2]))).
+    split.
+    - intros H0.
+      split...
+    - intros [H0 H1].
+      apply H.
+      intros x H2.
+      inversion H2; subst.
+      destruct H3 as [H3 | [H3 | []]]; subst...
+  Qed.
+
+  Lemma PrincipleOfTarski {D : Type} `{D_isCompleteLattice : isCompleteLattice D} :
+    forall f : monotonic_map (@CompleteLattice_requiresPoset D D_isCompleteLattice) (@CompleteLattice_requiresPoset D D_isCompleteLattice),
+    forall x : D,
+    x =< proj1_sig f x -> x =< proj1_sig (nu f).
+  Proof with eauto with *.
+    intros f x H.
+    unfold nu.
+    destruct (supremum_always_exists_in_CompleteLattice (fun x0 : D => x0 =< proj1_sig f x0)) as [gfp H0].
+    simpl.
+    apply H0...
+  Qed.
+
+  Lemma StrongCoinduction {D : Type} `{D_isCompleteLattice : isCompleteLattice D} :
+    forall f : monotonic_map (@CompleteLattice_requiresPoset D D_isCompleteLattice) (@CompleteLattice_requiresPoset D D_isCompleteLattice),
+    forall x : D,
+    x =< proj1_sig (nu f) <-> x =< proj1_sig f (or_plus x (proj1_sig (nu f))).
+  Proof with eauto with *.
+    intros f.
+    destruct (proj2_sig (nu f)) as [H H0].
+    assert (claim1 : forall x : D, proj1_sig f (proj1_sig (nu f)) =< proj1_sig f (or_plus x (proj1_sig (nu f)))).
+    { intros x.
+      apply (proj2_sig f).
+      apply le_or_plus.
+    }
+    intros x.
+    split.
+    - intros H1.
+      transitivity (proj1_sig (nu f))...
+    - intros H1.
+      enough (claim2 : or_plus x (proj1_sig (nu f)) =< proj1_sig f (or_plus x (proj1_sig (nu f)))).
+      { transitivity (proj1_sig f (or_plus x (proj1_sig (nu f))))...
+        apply PrincipleOfTarski.
+        apply (proj2_sig f)... 
+      }
+      apply or_plus_le_iff...
+  Qed.
+
+  Example G_f_aux_isMonotonic {D : Type} `{D_isCompleteLattice : isCompleteLattice D} :
+    forall f : monotonic_map (@CompleteLattice_requiresPoset D D_isCompleteLattice) (@CompleteLattice_requiresPoset D D_isCompleteLattice),
+    forall x : D,
+    isMonotonicMap (fun y : D => proj1_sig f (or_plus x y)).
+  Proof with eauto with *.
+    intros f d x1 x2 H.
+    apply (proj2_sig f).
+    apply or_plus_le_iff.
+    split.
+    - apply le_or_plus.
+    - transitivity x2...
+  Qed.
+
+  Definition G_f {D : Type} `{D_isCompleteLattice : isCompleteLattice D} : monotonic_map (@CompleteLattice_requiresPoset D D_isCompleteLattice) (@CompleteLattice_requiresPoset D D_isCompleteLattice) -> (D -> D) :=
+    fun f : monotonic_map (@CompleteLattice_requiresPoset D D_isCompleteLattice) (@CompleteLattice_requiresPoset D D_isCompleteLattice) =>
+    let G_f_aux : D -> D -> D := fun x : D => fun y : D => proj1_sig f (or_plus x y) in
+    fun x : D =>
+    proj1_sig (nu (exist _ (G_f_aux x) (G_f_aux_isMonotonic f x)))
+  .
+
+  Lemma G_f_isMonotoinc {D : Type} `{D_isCompleteLattice : isCompleteLattice D} :
+    forall f : monotonic_map (@CompleteLattice_requiresPoset D D_isCompleteLattice) (@CompleteLattice_requiresPoset D D_isCompleteLattice),
+    isMonotonicMap (G_f f).
+  Proof with eauto with *.
+    intros f.
+    set (G_f_aux := fun x : D => fun y : D => proj1_sig f (or_plus x y)).
+    intros x1 x2 H.
+    apply StrongCoinduction.
+    unfold nu.
+    simpl.
+    destruct (supremum_always_exists_in_CompleteLattice (fun y : D => y =< proj1_sig f (or_plus x2 y))) as [gfp2 H0].
+    simpl in *.
+    assert (claim1 : G_f f x1 == proj1_sig f (or_plus x1 (G_f f x1))) by apply (proj2_sig (nu (exist _ (G_f_aux x1) (G_f_aux_isMonotonic f x1)))).
+    transitivity (proj1_sig f (or_plus x1 (G_f f x1)))...
+    apply (proj2_sig f).
+    transitivity (or_plus x2 (G_f f x1)).
+    - apply or_plus_le_iff...
+    - apply or_plus_le_iff...
+  Qed.
+
+  Definition ParameterizedGreatestFixedpoint {D : Type} `{D_isCompleteLattice : isCompleteLattice D} : monotonic_map (@CompleteLattice_requiresPoset D D_isCompleteLattice) (@CompleteLattice_requiresPoset D D_isCompleteLattice) -> monotonic_map (@CompleteLattice_requiresPoset D D_isCompleteLattice) (@CompleteLattice_requiresPoset D D_isCompleteLattice) :=
+    fun f : monotonic_map (@CompleteLattice_requiresPoset D D_isCompleteLattice) (@CompleteLattice_requiresPoset D D_isCompleteLattice) =>
+    exist _ (G_f f) (G_f_isMonotoinc f)
+  .
+
+  Lemma ParameterizedGreatestFixedpoint_isMonotonic {D : Type} `{D_isCompleteLattice : isCompleteLattice D} :
+    @isMonotonicMap (monotonic_map (@CompleteLattice_requiresPoset D D_isCompleteLattice) (@CompleteLattice_requiresPoset D D_isCompleteLattice)) (monotonic_map (@CompleteLattice_requiresPoset D D_isCompleteLattice) (@CompleteLattice_requiresPoset D D_isCompleteLattice)) (MonotonicMap_can_be_pointwise_partially_ordered (@CompleteLattice_requiresPoset D D_isCompleteLattice) (@CompleteLattice_requiresPoset D D_isCompleteLattice)) (MonotonicMap_can_be_pointwise_partially_ordered (@CompleteLattice_requiresPoset D D_isCompleteLattice) (@CompleteLattice_requiresPoset D D_isCompleteLattice)) ParameterizedGreatestFixedpoint.
+  Proof with eauto with *.
+    intros f1 f2 H x.
+    simpl.
+    unfold G_f, nu.
+    simpl.
+    destruct (supremum_always_exists_in_CompleteLattice (fun y : D => y =< proj1_sig f1 (or_plus x y))) as [gfp1 H0].
+    destruct (supremum_always_exists_in_CompleteLattice (fun y : D => y =< proj1_sig f2 (or_plus x y))) as [gfp2 H1].
+    simpl.
+    apply H0.
+    unfold member.
+    intros y H2.
+    apply H1...
+  Qed.
+
+  Definition bot {D : Type} `{D_isCompleteLattice : isCompleteLattice D} : D :=
+    proj1_sig (supremum_always_exists_in_CompleteLattice empty)
+  .
+
+  Lemma bot_isBottom {D : Type} `{D_isCompleteLattice : isCompleteLattice D} :
+    forall x : D,
+    bot =< x.
+  Proof.
+    intros x.
+    apply (proj2_sig (supremum_always_exists_in_CompleteLattice empty)).
+    intros x' H.
+    inversion H; subst.
+    contradiction H0.
+  Qed.
+
+  Global Hint Resolve bot_isBottom : my_hints.
+
+  Lemma initialize_cofixpoint {D : Type} `{D_isCompleteLattice : isCompleteLattice D} :
+    forall f : monotonic_map (@CompleteLattice_requiresPoset D D_isCompleteLattice) (@CompleteLattice_requiresPoset D D_isCompleteLattice),
+    proj1_sig (nu f) == proj1_sig (ParameterizedGreatestFixedpoint f) bot.
+  Proof with eauto with *.
+    intros f.
+    symmetry.
+    unfold ParameterizedGreatestFixedpoint, G_f, nu.
+    simpl.
+    destruct (supremum_always_exists_in_CompleteLattice (fun y : D => y =< proj1_sig f (or_plus bot y))) as [gfp1 H].
+    destruct (supremum_always_exists_in_CompleteLattice (fun y : D => y =< proj1_sig f y)) as [gfp2 H0].
+    simpl.
+    apply Poset_asym.
+    - apply H.
+      intros x H1.
+      apply H0...
+      unfold member in *.
+      transitivity (proj1_sig f (or_plus bot x)).
+      + apply H1.
+      + apply (proj2_sig f).
+        apply or_plus_le_iff...
+    - apply H0.
+      intros x H1.
+      apply H...
+      unfold member in *.
+      transitivity (proj1_sig f x).
+      + apply H1.
+      + apply (proj2_sig f)...
+  Qed.
+
+  Lemma unfold_cofixpoint {D : Type} `{D_isCompleteLattice : isCompleteLattice D} :
+    forall f : monotonic_map (@CompleteLattice_requiresPoset D D_isCompleteLattice) (@CompleteLattice_requiresPoset D D_isCompleteLattice),
+    forall x : D,
+    proj1_sig (ParameterizedGreatestFixedpoint f) x == proj1_sig f (or_plus x (proj1_sig (ParameterizedGreatestFixedpoint f) x)).
+  Proof with eauto with *.
+    intros f x.
+    unfold ParameterizedGreatestFixedpoint.
+    simpl.
+    unfold G_f, nu.
+    simpl.
+    destruct (supremum_always_exists_in_CompleteLattice (fun y : D => y =< proj1_sig f (or_plus x y))) as [gfp1 H].
+    simpl.
+    assert (claim1 := GreatestFixedPointOfPoset (fun y : D => proj1_sig f (or_plus x y)) (G_f_aux_isMonotonic f x) gfp1 H).
+    apply claim1.
+  Qed.
+
+  Lemma accumulate_cofixpoint {D : Type} `{D_isCompleteLattice : isCompleteLattice D} :
+    forall f : monotonic_map (@CompleteLattice_requiresPoset D D_isCompleteLattice) (@CompleteLattice_requiresPoset D D_isCompleteLattice),
+    forall x : D,
+    forall y : D,
+    y =< proj1_sig (ParameterizedGreatestFixedpoint f) x <-> y =< proj1_sig (ParameterizedGreatestFixedpoint f) (or_plus x y).
+  Proof with eauto with *.
+    unfold ParameterizedGreatestFixedpoint.
+    simpl.
+    intros f.
+    split.
+    - intros H.
+      transitivity (G_f f x).
+      + apply H.
+      + apply G_f_isMonotoinc...
+    - intros H.
+      assert (claim1 : proj1_sig (ParameterizedGreatestFixedpoint f) (or_plus x y) == proj1_sig f (or_plus (or_plus x y) (G_f f (or_plus x y)))) by now apply unfold_cofixpoint.
+      assert (claim2 : proj1_sig f (or_plus (or_plus x y) (G_f f (or_plus x y))) =< proj1_sig f (or_plus x (G_f f (or_plus x y)))).
+      { apply (proj2_sig f).
+        apply or_plus_le_iff.
+        split.
+        - apply or_plus_le_iff...
+        - apply le_or_plus.
+      }
+      assert (claim3 : G_f f (or_plus x y) =< G_f f x).
+      { apply PrincipleOfTarski.
+        simpl.
+        transitivity (proj1_sig f (or_plus (or_plus x y) (G_f f (or_plus x y))))...
+      }
+      transitivity (G_f f (or_plus x y))...
+  Qed.
+
+(* [PROVE ME] 2021-07-05
+\begin{lstlisting}
+  Theorem KnasterTarski {D : Type} `{D_isPoset : isPoset D} :
+    forall f : D -> D,
+    isMonotonic f ->
+    forall fps : ensemble D,
+    isSubsetOf fps (fixed_points f) ->
+    {sup_fps : D | isSupremum sup_fps fps}.
+\end{lstlisting}
+*)
 
   Definition isDirected {D : Type} `{D_isPoset : isPoset D} : ensemble D -> Prop :=
     fun X : ensemble D =>
@@ -891,7 +1065,7 @@ Module DomainTheory.
   .
 
   Next Obligation.
-    destruct (supremum_always_exists empty) as [min_D H].
+    destruct (supremum_always_exists_in_CompleteLattice empty) as [min_D H].
     exists min_D.
     intros x.
     apply H.
@@ -901,7 +1075,7 @@ Module DomainTheory.
   Defined.
 
   Next Obligation.
-    apply supremum_always_exists.
+    apply supremum_always_exists_in_CompleteLattice.
   Defined.
 
   Global Program Instance ScottTopology_isTopologicalSpace {D : Type} (D_requiresCompletePartialOrder : isCompletePartialOrder D) : isTopologicalSpace D :=
@@ -944,1776 +1118,4 @@ Module DomainTheory.
       exists x...
   Qed.
 
-  Definition U {D : Type} `{D_isCompletePartialOrder : isCompletePartialOrder D} : D -> ensemble D :=
-    fun x : D =>
-    fun z : D =>
-    ~ z =< x
-  .
-
-  Global Hint Unfold U : my_hints.
-
-  Lemma U_x_isOpen {D : Type} `{D_isCompletePartialOrder : isCompletePartialOrder D} :
-    forall x : D,
-    isOpen (U x).
-  Proof with eauto with *.
-    intros x.
-    assert ( claim1 :
-      forall y : D,
-      forall z : D,
-      member y (U x) ->
-      y =< z ->
-      member z (U x)
-    ).
-    { intros y z H H0 H1.
-      contradiction H...
-    }
-    split...
-    intros X H sup_X H0 H1.
-    inversion H; subst.
-    assert (claim2 : ~ (forall x0 : D, x0 =< x \/ ~ member x0 X)).
-    { intros H4.
-      contradiction H1.
-      apply (proj2 (H0 x)).
-      intros x0 H5.
-      destruct (H4 x0); [apply H6 | contradiction].
-    }
-    apply not_all_ex_not in claim2.
-    destruct claim2 as [x1 H4].
-    exists x1.
-    apply not_or_and in H4.
-    destruct H4 as [H4 H5].
-    apply NNPP in H5...
-  Qed.
-
-  Definition characterization_of_ContinuousMap_on_cpos {D : Type} {D' : Type} `{D_isCompletePartialOrder : isCompletePartialOrder D} `{D'_isCompletePartialOrder : isCompletePartialOrder D'} : (D -> D') -> Prop :=
-    fun f : D -> D' =>
-    forall X : ensemble D,
-    isDirected X ->
-    let Y : ensemble D' := image f X in
-    exists sup_X : D, exists sup_Y : D', isSupremum sup_X X /\ isSupremum sup_Y Y /\ f sup_X = sup_Y
-  .
-
-  Lemma ContinuousMaps_on_cpos_are_always_monotonic {D : Type} {D' : Type} `{D_isCompletePartialOrder : isCompletePartialOrder D} `{D'_isCompletePartialOrder : isCompletePartialOrder D'} :
-    forall f : D -> D',
-    isContinuousMap f ->
-    forall x1 : D,
-    forall x2 : D,
-    x1 =< x2 ->
-    f x1 =< f x2.
-  Proof with eauto with *.
-    intros f H x1 x2 H0.
-    apply NNPP.
-    intros H1.
-    assert (H2 : member (f x1) (U (f x2))) by now unfold U.
-    assert (H3 : member x1 (preimage f (U (f x2)))) by now constructor.
-    assert (H4 : isOpen (preimage f (U (f x2)))) by now apply H, U_x_isOpen.
-    assert (H5 : member x2 (preimage f (U (f x2)))) by now apply (proj1 H4 x1 x2).
-    enough (H6 : member (f x2) (U (f x2)))...
-    inversion H5...
-  Qed.
-
-  Lemma ContinuousMaps_preservesDirected {D : Type} {D' : Type} `{D_isCompletePartialOrder : isCompletePartialOrder D} `{D'_isCompletePartialOrder : isCompletePartialOrder D'} :
-    forall f : D -> D',
-    isContinuousMap f ->
-    forall X : ensemble D,
-    isDirected X ->
-    isDirected (image f X).
-  Proof with eauto with *.
-    intros f H X H0.
-    destruct H0 as [H0 H1].
-    assert (H2 : forall x1 : D, forall x2 : D, x1 =< x2 -> f x1 =< f x2) by now apply ContinuousMaps_on_cpos_are_always_monotonic.
-    split.
-    - destruct H0 as [x0 H0]...
-    - intros y1 H3 y2 H4.
-      inversion H3; inversion H4; subst.
-      rename x into x1, x0 into x2.
-      destruct (H1 x1 H5 x2 H9) as [x3 [H6 [H7 H8]]].
-      exists (f x3).
-      repeat split...
-  Qed.
-
-  Lemma ContinuousMaps_preservesSupremum {D : Type} {D' : Type} `{D_isCompletePartialOrder : isCompletePartialOrder D} `{D'_isCompletePartialOrder : isCompletePartialOrder D'} :
-    forall f : D -> D',
-    isContinuousMap f ->
-    forall X : ensemble D,
-    isDirected X ->
-    forall sup_X : D,
-    isSupremum sup_X X ->
-    isDirected (image f X) ->
-    {sup_Y : D' | isSupremum sup_Y (image f X) /\ f sup_X = sup_Y}.
-  Proof with eauto with *.
-    intros f H X H0 sup_X H1 H2.
-    set (Y := image f X).
-    assert (H3 : forall x1 : D, forall x2 : D, x1 =< x2 -> f x1 =< f x2) by now apply ContinuousMaps_on_cpos_are_always_monotonic.
-    destruct (square_up_exists Y H2) as [sup_Y H4].
-    exists sup_Y.
-    assert (claim1 : sup_Y =< f sup_X).
-    { apply H4.
-      intros y H5.
-      inversion H5; subst.
-      apply H3, H1...
-    }
-    assert (claim2 : f sup_X =< sup_Y).
-    { apply NNPP.
-      intros H5.
-      assert (H6 : member (f sup_X) (U sup_Y)) by now unfold U.
-      assert (H7 : member sup_X (preimage f (U sup_Y))) by now constructor.
-      assert (H8 : isOpen (preimage f (U sup_Y))) by now apply H, U_x_isOpen.
-      destruct H8.
-      destruct (H9 X H0 sup_X H1 H7) as [x1 H10].
-      inversion H10; subst.
-      inversion H12; subst.
-      contradiction H13...
-    }
-    split...
-  Qed.
-
-  Theorem the_main_reason_for_introducing_ScottTopology {D : Type} {D' : Type} `{D_isCompletePartialOrder : isCompletePartialOrder D} `{D'_isCompletePartialOrder : isCompletePartialOrder D'} :
-    forall f : D -> D',
-    isContinuousMap f <-> characterization_of_ContinuousMap_on_cpos f.
-  Proof with eauto with *.
-    assert (claim1 : forall f : D -> D', isContinuousMap f -> forall x1 : D, forall x2 : D, x1 =< x2 -> f x1 =< f x2) by apply ContinuousMaps_on_cpos_are_always_monotonic.
-    split.
-    - intros H X H0.
-      inversion H0; subst.
-      set (Y := image f X).
-      assert (H3 : isDirected Y) by now apply ContinuousMaps_preservesDirected.
-      destruct (square_up_exists X H0) as [sup_X H4].
-      exists sup_X.
-      destruct (ContinuousMaps_preservesSupremum f H X H0 sup_X H4 H3) as [sup_Y H5].
-      exists sup_Y...
-    - intros H.
-      assert (claim2 : forall x1 : D, forall x2 : D, x1 =< x2 -> f x1 =< f x2).
-      { intros x1 x2 H0.
-        set (X := finite [x1; x2]).
-        set (Y := image f X).
-        assert (H1 : isSupremum x2 X).
-        { intros x.
-          split.
-          - intros H1 x' H2.
-            inversion H2; subst.
-            destruct H3 as [H3 | [H3 | []]]...
-          - intros H1...
-        }
-        assert (H2 : isDirected X).
-        { split.
-          - exists x1...
-          - intros x1' H2 x2' H3.
-            exists x2.
-            enough (x1' =< x2 /\ x2' =< x2)...
-        }
-        destruct (H X H2) as [sup_X H3].
-        destruct H3 as [sup_Y [H3 [H4 H5]]].
-        assert (H6 : sup_X = x2) by now apply (isSupremum_unique X).
-        subst...
-      }
-      intros O H0.
-      split.
-      + intros x1 x2 H1 H2.
-        inversion H1; subst.
-        constructor.
-        apply (proj1 H0 (f x1) (f x2))...
-      + intros X H1 sup_X H2 H3.
-        destruct (H X H1) as [sup_X' [sup_Y [H4 [H5 H6]]]].
-        assert (H7 : sup_X = sup_X') by now apply (isSupremum_unique X).
-        subst sup_X' sup_Y.
-        assert (H8 : member (f sup_X) O) by now inversion H3; subst.
-        assert (H9 : isDirected (image f X)).
-        { destruct H1 as [[x1_0 H1] H6].
-          split.
-          - exists (f x1_0)...
-          - intros y1 H10 y2 H11.
-            inversion H10; subst.
-            inversion H11; subst.
-            rename x into x1, x0 into x2.
-            destruct (H6 x1 H7 x2 H9) as [x3 [H12 [H13 H14]]].
-            exists (f x3).
-            repeat split...
-        }
-        assert (H10 : nonempty (intersection (image f X) O)).
-        { apply (proj2 H0 (image f X) H9 (f sup_X))...
-        }
-        destruct H10 as [y1 H10].
-        inversion H10; subst.
-        inversion H6; subst.
-        exists x...
-  Qed.
-
-  Local Program Instance DirectProductOfTwoPosets_isPoset {D : Type} {D' : Type} (D_requiresPoset : isPoset D) (D'_requiresPoset : isPoset D') : isPoset (D * D') :=
-    { leProp :=
-      fun p1 : (D * D') =>
-      fun p2 : (D * D') =>
-      fst p1 =< fst p2 /\ snd p1 =< snd p2
-    }
-  .
-
-  Next Obligation with eauto with *.
-    split.
-    - intros [x1 y1]...
-    - intros [x1 y1] [x2 y2] [x3 y3] [H H0] [H1 H2]...
-  Qed.
-
-  Next Obligation with eauto with *.
-    split.
-    - intros H.
-      subst.
-      repeat red.
-      repeat split...
-    - intros [[H H0] [H1 H2]].
-      apply injective_projections...
-  Qed.
-
-  Inductive getFsts {D : Type} {D' : Type} : ensemble (D * D') -> ensemble D :=
-  | in_getFsts {ps : ensemble (D * D')} :
-    forall x : D,
-    forall x' : D',
-    member (x, x') ps ->
-    member x (getFsts ps)
-  .
-
-  Global Hint Constructors getFsts : domain_theory_hints.
-
-  Inductive getSnds {D : Type} {D' : Type} : ensemble (D * D') -> ensemble D' :=
-  | in_getSnds {ps : ensemble (D * D')} :
-    forall x : D,
-    forall x' : D',
-    member (x, x') ps ->
-    member x' (getSnds ps)
-  .
-
-  Global Hint Constructors getSnds : domain_theory_hints.
-
-  Local Program Instance DirectProductOfTwoCompletePartialOrders_isCompletePartialOrder {D : Type} {D' : Type} (D_requiresCompletePartialOrder : isCompletePartialOrder D) (D'_requiresCompletePartialOrder : isCompletePartialOrder D') : isCompletePartialOrder (D * D') :=
-    { CompletePartialOrder_requiresPoset := DirectProductOfTwoPosets_isPoset (@CompletePartialOrder_requiresPoset D D_requiresCompletePartialOrder) (@CompletePartialOrder_requiresPoset D' D'_requiresCompletePartialOrder)
-    }
-  .
-
-  Next Obligation.
-    destruct (@bottom_exists D D_requiresCompletePartialOrder) as [bot_D H].
-    destruct (@bottom_exists D' D'_requiresCompletePartialOrder) as [bot_D' H0].
-    exists (bot_D, bot_D').
-    intros [d d'].
-    split; [apply H | apply H0].
-  Defined.
-
-  Next Obligation.
-    assert (claim1 : isDirected (getFsts X)).
-    { destruct H as [H H0].
-      split.
-      - destruct H as [[d0 d0'] H].
-        exists d0.
-        apply (in_getFsts d0 d0' H).
-      - intros d1 H1 d2 H2.
-        inversion H1; subst.
-        inversion H2; subst.
-        rename x' into d1', x'0 into d2'.
-        destruct (H0 (d1, d1') H3 (d2, d2') H4) as [[d3 d3'] [H5 [[H6 H7] [H8 H9]]]].
-        exists d3.
-        split.
-        + apply (in_getFsts d3 d3' H5).
-        + split; [apply H6 | apply H8].
-    }
-    assert (claim2 : isDirected (getSnds X)).
-    { destruct H as [H H0].
-      split.
-      - destruct H as [[d0 d0'] H].
-        exists d0'.
-        apply (in_getSnds d0 d0' H).
-      - intros d1' H1 d2' H2.
-        inversion H1; subst.
-        inversion H2; subst.
-        rename x into d1, x0 into d2.
-        destruct (H0 (d1, d1') H3 (d2, d2') H4) as [[d3 d3'] [H5 [[H6 H7] [H8 H9]]]].
-        exists d3'.
-        split.
-        + apply (in_getSnds d3 d3' H5).
-        + split; [apply H7 | apply H9].
-    }
-    destruct (@square_up_exists D D_requiresCompletePartialOrder (getFsts X) claim1) as [sup_X1 H0].
-    destruct (@square_up_exists D' D'_requiresCompletePartialOrder (getSnds X) claim2) as [sup_X2 H1].
-    exists (sup_X1, sup_X2).
-    intros [d d'].
-    split.
-    - intros H2 [x x'] H3.
-      split.
-      + apply H0.
-        * apply (proj1 H2).
-        * apply (in_getFsts x x' H3).
-      + apply H1.
-        * apply (proj2 H2).
-        * apply (in_getSnds x x' H3).
-    - intros H2.
-      split.
-      + apply H0.
-        intros x H3.
-        inversion H3; subst.
-        apply (proj1 (H2 (x, x') H4)).
-      + apply H1.
-        intros x' H3.
-        inversion H3; subst.
-        apply (proj2 (H2 (x, x') H4)).
-  Defined.
-
-  Local Notation "D1 ~> D2" := {f : D1 -> D2 | isContinuousMap f} (at level 70, no associativity) : type_scope.
-
-  Definition ContinuousMap_is_continuous {D : Type} {D' : Type} `{D_isCompletePartialOrder : isCompletePartialOrder D} `{D'_isCompletePartialOrder : isCompletePartialOrder D'} : forall f : D ~> D', isContinuousMap (proj1_sig f) :=
-    fun f : D ~> D' => proj2_sig f
-  .
-
-  Global Hint Resolve ContinuousMap_is_continuous : my_hints.
-
-  Lemma squigarrows_are_the_same_iff {D : Type} {D' : Type} `{D_isCompletePartialOrder : isCompletePartialOrder D} `{D'_isCompletePartialOrder : isCompletePartialOrder D'} :
-    forall f1 : D ~> D',
-    forall f2 : D ~> D',
-    (forall x : D, proj1_sig f1 x = proj1_sig f2 x) ->
-    f1 = f2.
-  Proof with eauto.
-    intros f1 f2 H.
-    enough (claim1 : proj1_sig f1 = proj1_sig f2) by apply (eq_sig f1 f2 claim1), proof_irrelevance.
-    apply functional_extensionality...
-  Qed.
-
-  Global Hint Resolve squigarrows_are_the_same_iff : my_hints.
-
-  Local Program Instance squigarrow_isPoset {D : Type} {D' : Type} (D_requiresCompletePartialOrder : isCompletePartialOrder D) (D'_requiresCompletePartialOrder : isCompletePartialOrder D') : isPoset (D ~> D') :=
-    { leProp :=
-      fun f1 : D ~> D' =>
-      fun f2 : D ~> D' =>
-      forall x : D,
-      proj1_sig f1 x =< proj1_sig f2 x
-    }
-  .
-
-  Next Obligation with eauto with *.
-    split...
-  Qed.
-
-  Next Obligation with eauto with *.
-    split.
-    - intros H.
-      subst.
-      split; intros x...
-    - intros [H H0]...
-  Qed.
-
-  Lemma sup_of_squigarrow_is_well_defined {D : Type} {D' : Type} `{D_isCompletePartialOrder : isCompletePartialOrder D} `{D'_isCompletePartialOrder : isCompletePartialOrder D'} :
-    forall fs : ensemble (D ~> D'),
-    isDirected fs ->
-    forall x : D,
-    isDirected (image (fun f : D ~> D' => proj1_sig f x) fs).
-  Proof with eauto with *.
-    intros fs [H H0] x.
-    split.
-    - destruct H as [f0].
-      exists (proj1_sig f0 x).
-      apply (in_image (fun f : D ~> D' => proj1_sig f x))...
-    - intros y1 H1 y2 H2.
-      inversion H1; subst.
-      inversion H2; subst.
-      rename x0 into f1, x1 into f2.
-      destruct (H0 f1 H3 f2 H4) as [f3 [H5 [H6 H7]]].
-      exists (proj1_sig f3 x).
-      repeat split...
-      apply (in_image (fun f : D ~> D' => proj1_sig f x))...
-  Qed.
-
-  Lemma sup_of_set_of_squigarrows_exists_if_it_is_directed {D : Type} {D' : Type} `{D_isCompletePartialOrder : isCompletePartialOrder D} `{D'_isCompletePartialOrder : isCompletePartialOrder D'} :
-    forall fs : ensemble (D ~> D'),
-    forall fs_isDirected : isDirected fs,
-    let f : D -> D' := fun x : D => proj1_sig (square_up_exists (image (fun f_i : D ~> D' => proj1_sig f_i x) fs) (sup_of_squigarrow_is_well_defined fs fs_isDirected x)) in
-    isContinuousMap f.
-  Proof with eauto with *.
-    intros fs H f.
-    apply the_main_reason_for_introducing_ScottTopology.
-    intros X H0 Y.
-    destruct (square_up_exists X H0) as [sup_X H1].
-    exists sup_X, (f sup_X).
-    assert ( claim1 :
-      forall f_i : D ~> D',
-      member f_i fs ->
-      isSupremum (proj1_sig f_i sup_X) (image (fun x : D => proj1_sig f_i x) X)
-    ).
-    { intros f_i H2.
-      assert (H3 : isContinuousMap (proj1_sig f_i))...
-      assert (H4 : characterization_of_ContinuousMap_on_cpos (proj1_sig f_i)) by now apply the_main_reason_for_introducing_ScottTopology.
-      destruct (H4 X H0) as [sup_X' [sup_Y' [H5 [H6 H7]]]].
-      assert (H8 : sup_X' = sup_X) by now apply (isSupremum_unique X).
-      subst...
-    }
-    assert (claim2 : isSupremum (f sup_X) (image (fun f_i : D ~> D' => proj1_sig f_i sup_X) fs)) by apply (proj2_sig (square_up_exists (image (fun f_i : D ~> D' => proj1_sig f_i sup_X) fs) (sup_of_squigarrow_is_well_defined fs H sup_X))).
-    assert (claim3 : isSupremum (f sup_X) (unions (image (fun f_i : D ~> D' => image (fun x : D => proj1_sig f_i x) X) fs))).
-    { apply isSupremum_unions_Xs_iff_isSupremum_image_sup_Xs.
-      - intros ys H2.
-        inversion H2; subst.
-        rename x into f_i.
-        exists (proj1_sig f_i sup_X)...
-      - intros y.
-        split.
-        + intros H2 y' [ys [H3 H4]].
-          inversion H3; subst.
-          rename x into f_i.
-          assert (H6 := claim1 f_i H5).
-          assert (H7 : y' = proj1_sig f_i sup_X) by now apply (isSupremum_unique (image (fun x : D => proj1_sig f_i x) X)).
-          transitivity (proj1_sig f_i sup_X)...
-          apply claim2...
-          apply (in_image (fun f_i0 : D ~> D' => proj1_sig f_i0 sup_X))...
-        + intros H2.
-          apply claim2.
-          intros y' H3.
-          inversion H3; subst.
-          rename x into f_i.
-          apply H2.
-          exists (image (fun x : D => proj1_sig f_i x) X).
-          split...
-          apply (in_image (fun f_i0 : D ~> D' => image (fun x : D => proj1_sig f_i0 x) X))...
-    }
-    assert (claim4 : isSupremum (f sup_X) (unions (image (fun x : D => image (fun f_i : D ~> D' => proj1_sig f_i x) fs) X))).
-    { enough (H2 : forall x' : D', member x' (unions (image (fun f_i : D ~> D' => image (fun x : D => proj1_sig f_i x) X) fs)) <-> member x' (unions (image (fun x : D => image (fun f_i : D ~> D' => proj1_sig f_i x) fs) X))) by now apply (proj2 (isSupremum_ext _ _ H2 _ claim3 _) eq_refl).
-      intros y.
-      split.
-      - intros H2.
-        inversion H2; subst.
-        rename xs into ys.
-        inversion H4; subst.
-        rename x into f_i.
-        inversion H3; subst.
-        apply (in_unions (image (fun f_i' : D ~> D' => proj1_sig f_i' x) fs)).
-        + apply (in_image (fun f_i' : D ~> D' => proj1_sig f_i' x))...
-        + apply (in_image (fun x0 : D => image (fun f_i0 : D ~> D' => proj1_sig f_i0 x0) fs))...
-      - intros H2.
-        inversion H2; subst.
-        rename xs into ys.
-        inversion H4; subst.
-        inversion H3; subst.
-        rename x0 into f_i.
-        apply (in_unions (image (fun x' : D => proj1_sig f_i x') X)).
-        + apply (in_image (fun x' : D => proj1_sig f_i x'))...
-        + apply (in_image (fun f_i0 : D ~> D' => image (fun x0 : D => proj1_sig f_i0 x0) X))...
-    }
-    assert (claim5 : isSupremum (f sup_X) (image_sup (image (fun x : D => image (fun f_i : D ~> D' => proj1_sig f_i x) fs) X))).
-    { apply isSupremum_unions_Xs_iff_isSupremum_image_sup_Xs...
-      intros ys H2.
-      inversion H2; subst.
-      exists (f x).
-      intros y.
-      split.
-      - intros H4 y' H5.
-        inversion H5; subst.
-        rename x0 into f_i.
-        apply (proj2_sig (square_up_exists (image (fun f_i : D ~> D' => proj1_sig f_i x) fs) (sup_of_squigarrow_is_well_defined fs H x)))...
-      - intros H4.
-        assert (H5 : isSupremum (f x) (image (fun f_i : D ~> D' => proj1_sig f_i x) fs)) by apply (proj2_sig (square_up_exists (image (fun f_i : D ~> D' => proj1_sig f_i x) fs) (sup_of_squigarrow_is_well_defined fs H x))).
-        apply H5...
-    }
-    assert (claim6 : isSupremum (f sup_X) (image f X)).
-    { intros y.
-      split.
-      - intros H2 y' H3.
-        inversion H3; subst.
-        apply claim5...
-        exists (image (fun f_i : D ~> D' => proj1_sig f_i x) fs).
-        split.
-        + apply (in_image (fun x0 : D => image (fun f_i : D ~> D' => proj1_sig f_i x0) fs))...
-        + apply (proj2_sig (square_up_exists (image (fun f_i : D ~> D' => proj1_sig f_i x) fs) (sup_of_squigarrow_is_well_defined fs H x))).
-      - intros H2.
-        apply claim5.
-        intros y' [ys [H3 H4]].
-        inversion H3; subst.
-        assert (H6 : isSupremum (f x) (image (fun f_i : D ~> D' => proj1_sig f_i x) fs)) by apply (proj2_sig (square_up_exists (image (fun f_i : D ~> D' => proj1_sig f_i x) fs) (sup_of_squigarrow_is_well_defined fs H x))).
-        assert (H7 : y' = f x) by now apply (isSupremum_unique (image (fun f_i : D ~> D' => proj1_sig f_i x) fs)).
-        transitivity (f x)...
-    }
-    split...
-  Qed.
-
-  Local Program Instance squigarrow_isCompletePartialOrder {D : Type} {D' : Type} (D_requiresCompletePartialOrder : isCompletePartialOrder D) (D'_requiresCompletePartialOrder : isCompletePartialOrder D') : isCompletePartialOrder (D ~> D') :=
-    { CompletePartialOrder_requiresPoset := squigarrow_isPoset D_requiresCompletePartialOrder D'_requiresCompletePartialOrder
-    }
-  .
-
-  Next Obligation.
-    set (bot := fun _ : D => proj1_sig bottom_exists).
-    assert (claim1 : isContinuousMap bot).
-    { intros Y [H H0].
-      split.
-      - intros x1 x2 H1 H2.
-        inversion H1; subst.
-        apply (in_preimage bot).
-        apply (H (bot x1) (bot x2) H3 (Poset_refl (proj1_sig bottom_exists))).
-      - intros X [[x_0 H1] H2] sup_X H3 H4.
-        inversion H4; subst.
-        exists x_0.
-        constructor.
-        + apply H1.
-        + apply (in_preimage bot).
-          apply (H (bot sup_X) (bot x_0) H5).
-          apply Poset_refl.
-    }
-    exists (exist _ bot claim1).
-    simpl.
-    intros f x.
-    apply (proj2_sig bottom_exists).
-  Defined.
-
-  Next Obligation.
-    rename X into fs, H into fs_isDirected.
-    set (sup_fs := fun x : D => proj1_sig (square_up_exists (image (fun f_i : D ~> D' => proj1_sig f_i x) fs) (sup_of_squigarrow_is_well_defined fs fs_isDirected x))).
-    exists (exist _ sup_fs (sup_of_set_of_squigarrows_exists_if_it_is_directed fs fs_isDirected)).
-    assert (claim1 : forall x : D, isSupremum (sup_fs x) (image (fun f_i : D ~> D' => proj1_sig f_i x) fs)) by apply (fun x : D => proj2_sig (square_up_exists (image (fun f_i : D ~> D' => proj1_sig f_i x) fs) (sup_of_squigarrow_is_well_defined fs fs_isDirected x))).
-    intros f.
-    simpl.
-    split.
-    - intros H f' H0 x.
-      apply (claim1 x).
-      + apply H.
-      + apply (in_image (fun f_i : D ~> D' => proj1_sig f_i x)).  
-        apply H0.
-    - intros H x.
-      apply (claim1 x).
-      intros f' H0.
-      inversion H0; subst.
-      rename x0 into f'.
-      apply (H f').
-      apply H1.
-  Defined.
-
-  Lemma separately_continuous_iff {D1 : Type} {D2 : Type} {D3 : Type} `{D1_isCompletePartialOrder : isCompletePartialOrder D1} `{D2_isCompletePartialOrder : isCompletePartialOrder D2} `{D3_isCompletePartialOrder : isCompletePartialOrder D3} :
-    forall f : D1 * D2 -> D3,
-    ((forall x1 : D1, isContinuousMap (fun x2 : D2 => f (x1, x2))) /\ (forall x2 : D2, isContinuousMap (fun x1 : D1 => f (x1, x2)))) <-> isContinuousMap f.
-  Proof with eauto with *.
-    intros f.
-    split.
-    - intros [H H0].
-      apply the_main_reason_for_introducing_ScottTopology.
-      intros X H1 Y.
-      destruct (square_up_exists X H1) as [[sup_X1 sup_X2] H2].
-      set (X1 := getFsts X).
-      set (X2 := getSnds X).
-      exists (sup_X1, sup_X2), (f (sup_X1, sup_X2)).
-      assert (claim1 : isDirected X1).
-      { destruct H1 as [[[x1_0 x2_0] H1] H3].
-        split.
-        - exists x1_0.
-          apply (in_getFsts x1_0 x2_0)...
-        - intros x1_1 H4 x1_2 H5.
-          inversion H4; subst.
-          inversion H5; subst.
-          rename x' into x2_1, x'0 into x2_2.
-          destruct (H3 (x1_1, x2_1) H6 (x1_2, x2_2) H7) as [[x3_1 x3_2] [H8 [[H9 H10] [H11 H12]]]].
-          exists x3_1.
-          split...
-          apply (in_getFsts x3_1 x3_2)...
-      }
-      assert (claim2 : isDirected X2).
-      { destruct H1 as [[[x1_0 x2_0] H1] H3].
-        split.
-        - exists x2_0.
-          apply (in_getSnds x1_0 x2_0)...
-        - intros x2_1 H4 x2_2 H5.
-          inversion H4; subst.
-          inversion H5; subst.
-          rename x into x1_1, x0 into x1_2.
-          destruct (H3 (x1_1, x2_1) H6 (x1_2, x2_2) H7) as [[x3_1 x3_2] [H8 [[H9 H10] [H11 H12]]]].
-          exists x3_2.
-          split...
-          apply (in_getSnds x3_1 x3_2)...
-      }
-      assert ( claim3 :
-        forall x1 : D1,
-        exists sup_X2_x1 : D2, exists sup_f_X2_x1 : D3, isSupremum sup_X2_x1 X2 /\ isSupremum sup_f_X2_x1 (image (fun x2 : D2 => f (x1, x2)) X2) /\ f (x1, sup_X2_x1) = sup_f_X2_x1
-      ).
-      { intros x1.
-        apply (the_main_reason_for_introducing_ScottTopology (fun x2 : D2 => f (x1, x2)))...
-      }
-      assert ( claim4 :
-        forall x2 : D2,
-        exists sup_X1_x2 : D1, exists sup_f_X1_x2 : D3, isSupremum sup_X1_x2 X1 /\ isSupremum sup_f_X1_x2 (image (fun x1 : D1 => f (x1, x2)) X1) /\ f (sup_X1_x2, x2) = sup_f_X1_x2
-      ).
-      { intros x2.
-        apply (the_main_reason_for_introducing_ScottTopology (fun x1 : D1 => f (x1, x2)))...
-      }
-      assert (XXX : isSupremum sup_X1 X1 /\ isSupremum sup_X2 X2).
-      { destruct (square_up_exists X1 claim1) as [sup_X1' H3].
-        destruct (square_up_exists X2 claim2) as [sup_X2' H4].
-        assert (H5 : isSupremum (sup_X1', sup_X2') X).
-        { intros [x1 x2].
-          split.
-          - intros [H5 H6] [x1' x2'] H7.
-            simpl in *.
-            split.
-            + apply H3...
-              apply (in_getFsts x1' x2')...
-            + apply H4...
-              apply (in_getSnds x1' x2')...
-          - intros H5.
-            split.
-            + apply H3.
-              intros x1' H6.
-              inversion H6; subst.
-              rename x' into x2'.
-              apply (proj1 (H5 (x1', x2') H7)).
-            + apply H4.
-              intros x2' H6.
-              inversion H6; subst.
-              rename x into x1'.
-              apply (proj2 (H5 (x1', x2') H7)).
-          }
-        assert (H6 : (sup_X1, sup_X2) = (sup_X1', sup_X2')) by now apply (isSupremum_unique X).
-        inversion H6; subst.
-        simpl in *.
-        split...
-      }
-      destruct XXX as [claim5 claim6].
-      assert (claim7 : isSupremum (f (sup_X1, sup_X2)) (image (fun x2 : D2 => f (sup_X1, x2)) X2)).
-      { destruct (claim3 sup_X1) as [sup_X2_x1 [sup_f_X1_x2 [H3 [H4 H5]]]].
-        assert (H6 : isSupremum (f (sup_X1, sup_X2)) (image (fun x2 : D2 => f (sup_X1, x2)) X2) <-> sup_f_X1_x2 = f (sup_X1, sup_X2)) by now apply (@isSupremum_unique D3 (@CompletePartialOrder_requiresPoset D3 D3_isCompletePartialOrder)).
-        apply H6.
-        transitivity (f (sup_X1, sup_X2_x1)).
-        - symmetry...
-        - enough (H7 : sup_X2_x1 = sup_X2) by congruence.
-          apply (isSupremum_unique X2)...
-      }
-      assert ( claim8 :
-        forall x2 : D2,
-        member x2 X2 ->
-        isSupremum (f (sup_X1, x2)) (image (fun x1 : D1 => f (x1, x2)) X1)
-      ).
-      { intros x2 H3.
-        destruct (claim4 x2) as [sup_X1' [sup_f_X1_x2' [H4 [H5 H6]]]].
-        assert (H7 : isSupremum (f (sup_X1, x2)) (image (fun x1 : D1 => f (x1, x2)) X1) <-> sup_f_X1_x2' = f (sup_X1, x2)) by now apply (@isSupremum_unique D3 (@CompletePartialOrder_requiresPoset D3 D3_isCompletePartialOrder)).
-        apply H7.
-        transitivity (f (sup_X1', x2)).
-        - symmetry...
-        - enough (H8 : sup_X1' = sup_X1) by congruence.
-          apply (isSupremum_unique X1)...
-      }
-      assert (claim9 : isSupremum (f (sup_X1, sup_X2)) (image_sup (image (fun x2 : D2 => image (fun x1 : D1 => f (x1, x2)) X1) X2))).
-      { intros y.
-        split.
-        - intros H3 y' [ys [H4 H5]].
-          inversion H4; subst.
-          rename x into x2.
-          assert (H7 : isSupremum (f (sup_X1, x2)) (image (fun x1 : D1 => f (x1, x2)) X1)) by now apply claim8.
-          assert (H8 : y' = (f (sup_X1, x2))) by now apply (isSupremum_unique (image (fun x1 : D1 => f (x1, x2)) X1)).
-          assert (H9 : f (sup_X1, x2) =< f (sup_X1, sup_X2)).
-          { apply (ContinuousMaps_on_cpos_are_always_monotonic (fun x2' : D2 => f (sup_X1, x2')) (H sup_X1)).
-            apply claim6...
-          }
-          transitivity (f (sup_X1, x2))...
-        - intros H7.
-          apply claim7.
-          intros y' H8.
-          inversion H8; subst.
-          rename x into x2.
-          apply H7...
-          exists (image (fun x1 : D1 => f (x1, x2)) X1).
-          split.
-          + apply (in_image (fun x0 : D2 => image (fun x1 : D1 => f (x1, x0)) X1))...
-          + apply claim8...
-      }
-      assert (claim10 : isSupremum (f (sup_X1, sup_X2)) (unions (image (fun x2 : D2 => image (fun x1 : D1 => f (x1, x2)) X1) X2))).
-      { apply isSupremum_unions_Xs_iff_isSupremum_image_sup_Xs...
-        intros ys H3.
-        inversion H3; subst.
-        rename x into x2.
-        exists (f (sup_X1, x2))...
-      }
-      assert (claim11 : isSupremum (f (sup_X1, sup_X2)) (image f X)).
-      { intros y.
-        split.
-        - intros H3 y' H4.
-          inversion H4; subst.
-          apply claim10.
-          + apply H3.
-          + destruct x as [x1 x2].
-            apply (in_unions (image (fun x1' : D1 => f (x1', x2)) X1)).
-            * apply (in_image (fun x1' : D1 => f (x1', x2))).
-              apply (in_getFsts x1 x2)...
-            * apply (in_image (fun x0 : D2 => image (fun x3 : D1 => f (x3, x0)) X1)).
-              apply (in_getSnds x1 x2)...
-        - intros H3.
-          apply claim10.
-          intros y' H4.
-          inversion H4; subst.
-          rename xs into ys.
-          inversion H6; subst.
-          rename x into x2_2.
-          inversion H5; subst.
-          rename x into x1_1.
-          inversion H8; subst.
-          rename x' into x2_1.
-          inversion H7; subst.
-          rename x into x1_2.
-          destruct H1 as [H1 H11].
-          destruct (H11 (x1_1, x2_1) H9 (x1_2, x2_2) H10) as [[x3_1 x3_2] [H12 [[H13 H14] [H15 H16]]]].
-          simpl in *.
-          assert (H17 : f (x1_1, x2_2) =< f (x3_1, x3_2)).
-          { transitivity (f (x1_1, x3_2)).
-            - apply (ContinuousMaps_on_cpos_are_always_monotonic (fun x2 : D2 => f (x1_1, x2)))...
-            - apply (ContinuousMaps_on_cpos_are_always_monotonic (fun x1 : D1 => f (x1, x3_2)))...
-          }
-          transitivity (f (x3_1, x3_2))...
-      }
-      split...
-    - intros H.
-      split.
-      + intros x1.
-        apply (the_main_reason_for_introducing_ScottTopology (fun x2 : D2 => f (x1, x2))).
-        intros X2 H0 Y.
-        destruct (square_up_exists X2 H0) as [sup_X2 H1].
-        set (X := image (fun x2 : D2 => (x1, x2)) X2).
-        assert (claim1 : isDirected X).
-        { destruct H0 as [[x2_0 H0] H2].
-          split.
-          - exists (x1, x2_0).
-            apply (in_image (fun x2 : D2 => (x1, x2)))...
-          - intros [x1_1 x2_1] H3 [x1_2 x2_2] H4.
-            inversion H3; subst x1_1; subst.
-            inversion H4; subst x1_2; subst.
-            rename H8 into H5, H9 into H6.
-            destruct (H2 x2_1 H5 x2_2 H6) as [x3_2 [H7 [H8 H9]]].
-            exists (x1, x3_2).
-            repeat split...
-        }
-        destruct (square_up_exists X claim1) as [sup_X H2].
-        exists sup_X2, (f sup_X).
-        assert (claim2 : (x1, sup_X2) = sup_X).
-        { apply (isSupremum_unique X)...
-          intros [x_1 x_2].
-          split.
-          - intros [H3 H4] [x_1' x_2'] H5.
-            inversion H5; subst x_1'; subst.
-            simpl.
-            split...
-          - intros H3.
-            simpl.
-            split.
-            + destruct H0 as [[x2_0 H0] H4].
-              apply (H3 (x1, x2_0))...
-            + apply H1.
-              intros x_2' H4.
-              apply (H3 (x1, x_2'))...
-        }
-        assert (claim3 : f (x1, sup_X2) = f sup_X) by congruence.
-        assert (XXX : exists sup_X' : D1 * D2, exists sup_Y' : D3, isSupremum sup_X' X /\ isSupremum sup_Y' (image f X) /\ f sup_X' = sup_Y') by now apply the_main_reason_for_introducing_ScottTopology.
-        destruct XXX as [sup_X' [sup_Y' [H3 [H4 H5]]]].
-        assert (claim4 : isSupremum (f sup_X) Y).
-        { assert (H6 : isSupremum (f sup_X) (image f X) <-> sup_Y' = f sup_X) by now apply (@isSupremum_unique D3 (@CompletePartialOrder_requiresPoset D3 D3_isCompletePartialOrder) (image f X)).
-          assert (H7 : isSupremum (f sup_X) (image f X)).
-          { apply H6.
-            transitivity (f sup_X').
-            - symmetry...
-            - enough (H7 : sup_X' = sup_X) by congruence.
-              apply (isSupremum_unique X)...
-          }
-          assert (H8 : forall y : D3, member y (image f X) <-> member y Y).
-          { intros y.
-            split.
-            - intros H8.
-              inversion H8; subst.
-              inversion H9; subst.
-              rename x0 into x2.
-              apply (in_image (fun x2 : D2 => f (x1, x2)))...
-            - intros H8.
-              inversion H8; subst.
-              rename x into x2.
-              apply (in_image f)...
-          }
-          apply (proj2 (@isSupremum_ext D3 (@CompletePartialOrder_requiresPoset D3 D3_isCompletePartialOrder) _ _ H8 _ H7 _) eq_refl).
-        }
-        split...
-      + intros x2.
-        apply (the_main_reason_for_introducing_ScottTopology (fun x1 : D1 => f (x1, x2))).
-        intros X1 H0 Y.
-        destruct (square_up_exists X1 H0) as [sup_X1 H1].
-        set (X := image (fun x1 : D1 => (x1, x2)) X1).
-        assert (YYY : forall x1 : D1, member x1 X1 -> member (x1, x2) X).
-        { intros x1 H2.
-          apply (in_image (fun x1 : D1 => (x1, x2))), H2.
-        }
-        assert (claim1 : isDirected X).
-        { destruct H0 as [[x1_0 H0] H2].
-          split.
-          - exists (x1_0, x2).
-            apply (in_image (fun x1 : D1 => (x1, x2)))...
-          - intros [x1_1 x2_1] H3 [x1_2 x2_2] H4.
-            inversion H3; subst x2_1; subst.
-            inversion H4; subst x2_2; subst.
-            rename H8 into H5, H9 into H6.
-            destruct (H2 x1_1 H5 x1_2 H6) as [x3_1 [H7 [H8 H9]]].
-            exists (x3_1, x2).
-            repeat split...
-        }
-        destruct (square_up_exists X claim1) as [sup_X H2].
-        exists sup_X1, (f sup_X).
-        assert (claim2 : (sup_X1, x2) = sup_X).
-        { apply (isSupremum_unique X)...
-          intros [x_1 x_2].
-          split.
-          - intros [H3 H4] [x_1' x_2'] H5.
-            inversion H5; subst x_1'; subst.
-            simpl.
-            split...
-          - intros H3.
-            simpl.
-            split.
-            + apply H1.
-              intros x_1' H4.
-              apply (H3 (x_1', x2))...
-            + destruct H0 as [[x1_0 H0] H4].
-              apply (H3 (x1_0, x2))...
-        }
-        assert (claim3 : f (sup_X1, x2) = f sup_X) by congruence.
-        assert (XXX : exists sup_X' : D1 * D2, exists sup_Y' : D3, isSupremum sup_X' X /\ isSupremum sup_Y' (image f X) /\ f sup_X' = sup_Y') by now apply the_main_reason_for_introducing_ScottTopology.
-        destruct XXX as [sup_X' [sup_Y' [H3 [H4 H5]]]].
-        assert (claim4 : isSupremum (f sup_X) Y).
-        { assert (H6 : isSupremum (f sup_X) (image f X) <-> sup_Y' = f sup_X) by now apply (@isSupremum_unique D3 (@CompletePartialOrder_requiresPoset D3 D3_isCompletePartialOrder) (image f X)).
-          assert (H7 : isSupremum (f sup_X) (image f X)).
-          { apply H6.
-            transitivity (f sup_X').
-            - symmetry...
-            - enough (H7 : sup_X' = sup_X) by congruence.
-              apply (isSupremum_unique X)...
-          }
-          assert (H8 : forall y : D3, member y (image f X) <-> member y Y).
-          { intros y.
-            split.
-            - intros H8.
-              inversion H8; subst.
-              inversion H9; subst.
-              rename x0 into x1.
-              apply (in_image (fun x1 : D1 => f (x1, x2)))...
-            - intros H8.
-              inversion H8; subst.
-              rename x into x1.
-              apply (in_image f)...
-          }
-          apply (proj2 (@isSupremum_ext D3 (@CompletePartialOrder_requiresPoset D3 D3_isCompletePartialOrder) _ _ H8 _ H7 _) eq_refl).
-        }
-        split...
-  Qed.
-
-  Definition ScottApp {D : Type} {D' : Type} `{D_isCompletePartialOrder : isCompletePartialOrder D} `{D'_isCompletePartialOrder : isCompletePartialOrder D'} : (D ~> D') * D -> D' :=
-    @uncurry (D ~> D') D D' (@proj1_sig (D -> D') isContinuousMap)
-  .
-
-  Lemma ScottApp_isContinuousMap {D : Type} {D' : Type} `{D_isCompletePartialOrder : isCompletePartialOrder D} `{D'_isCompletePartialOrder : isCompletePartialOrder D'} :
-    isContinuousMap (@ScottApp D D' _ _).
-  Proof with eauto with *.
-    apply separately_continuous_iff.
-    split.
-    - unfold ScottApp...
-    - intros x.
-      apply the_main_reason_for_introducing_ScottTopology.
-      intros fs fs_isDirected Y.
-      set (f := fun x : D => proj1_sig (square_up_exists (image (fun f_i : D ~> D' => proj1_sig f_i x) fs) (sup_of_squigarrow_is_well_defined fs fs_isDirected x))).
-      set (sup_fs := exist isContinuousMap f (sup_of_set_of_squigarrows_exists_if_it_is_directed fs fs_isDirected)).
-      assert (claim1 : forall x : D, isSupremum (f x) (image (fun f_i : D ~> D' => proj1_sig f_i x) fs)) by apply (fun x : D => proj2_sig (square_up_exists (image (fun f_i : D ~> D' => proj1_sig f_i x) fs) (sup_of_squigarrow_is_well_defined fs fs_isDirected x))).
-      assert (claim2 : isSupremum sup_fs fs).
-      { intros g.
-        simpl.
-        split.
-        - intros H g' H0 x'.
-          apply (claim1 x')...
-          apply (in_image (fun f_i : D ~> D' => proj1_sig f_i x'))...  
-        - intros H x'.
-          apply (claim1 x').
-          intros g' H0.
-          inversion H0; subst.
-          rename x0 into g'.
-          apply (H g')...
-      }
-      exists sup_fs, (ScottApp (sup_fs, x)).
-      assert (claim3 : isSupremum (ScottApp (sup_fs, x)) Y).
-      { intros y.
-        split.
-        - intros H y' H0.
-          apply (claim1 x)...
-        - intros H.
-          apply (claim1 x)...
-      }
-      split...
-  Qed.
-
 End DomainTheory.
-
-Module UntypedLamdbdaCalculus.
-
-  Import ListNotations.
-
-  Import MyUtilities.
-
-  Import MyStructures.
-
-  Import MyEnsemble.
-
-  Import GeneralTopology.
-
-  Import DomainTheory.
-
-  Definition ivar : Set :=
-    nat
-  .
-
-  Definition ivar_eq_dec :
-    forall x : ivar,
-    forall y : ivar,
-    {x = y} + {x <> y}.
-  Proof.
-    apply Nat.eq_dec.
-  Defined.
-
-  Inductive tm : Set :=
-  | tmVar : forall x : ivar, tm
-  | tmApp : forall P1 : tm, forall P2 : tm, tm
-  | tmLam : forall y : ivar, forall Q : tm, tm
-  .
-
-  Definition tm_eq_dec :
-    forall M1 : tm,
-    forall M2 : tm,
-    {M1 = M2} + {M1 <> M2}.
-  Proof with try ((left; congruence) || (right; congruence)).
-    induction M1; destruct M2...
-    - destruct (ivar_eq_dec x x0)...
-    - destruct (IHM1_1 M2_1); destruct (IHM1_2 M2_2)...
-    - destruct (ivar_eq_dec y y0); destruct (IHM1 M2)...
-  Defined.
-
-  Fixpoint getRank (M : tm) {struct M} : nat :=
-    match M with
-    | tmVar x => 0
-    | tmApp P1 P2 => S (max (getRank P1) (getRank P2))
-    | tmLam y Q => S (getRank Q)
-    end
-  .
-
-  Inductive subtm : tm -> tm -> Set :=
-  | subtmRefl : forall M : tm, subtm M M
-  | subtmAppL : forall M : tm, forall P1 : tm, forall P2 : tm, subtm M P1 -> subtm M (tmApp P1 P2)
-  | subtmAppR : forall M : tm, forall P1 : tm, forall P2 : tm, subtm M P2 -> subtm M (tmApp P1 P2)
-  | subtmLAbs : forall M : tm, forall y : ivar, forall Q : tm, subtm M Q -> subtm M (tmLam y Q)
-  .
-
-  Global Hint Constructors tm : my_hints.
-
-  Lemma subtm_getRank :
-    forall M : tm,
-    forall N : tm,
-    subtm M N ->
-    getRank M <= getRank N.
-  Proof with lia.
-    intros M N X.
-    induction X; simpl...
-  Qed.
-
-  Lemma subtm_and_same_rank_implies_same_term :
-    forall M : tm,
-    forall N : tm,
-    subtm M N ->
-    getRank M = getRank N ->
-    M = N.
-  Proof with lia.
-    intros M N X.
-    destruct X; intros.
-    - reflexivity.
-    - assert (H0 := subtm_getRank M P1 X).
-      simpl in *...
-    - assert (H0 := subtm_getRank M P2 X).
-      simpl in *...
-    - assert (H0 := subtm_getRank M Q X).
-      simpl in *...
-  Qed.
-
-  Lemma subtm_refl :
-    forall M1 : tm,
-    subtm M1 M1.
-  Proof.
-    apply subtmRefl.
-  Qed.
-
-  Local Hint Resolve subtm_refl : core.
-
-  Lemma subtm_asym :
-    forall M1 : tm,
-    forall M2 : tm,
-    subtm M1 M2 ->
-    subtm M2 M1 ->
-    M1 = M2.
-  Proof with eauto.
-    intros.
-    apply subtm_and_same_rank_implies_same_term...
-    enough (getRank M1 <= getRank M2 /\ getRank M2 <= getRank M1) by lia.
-    split; apply subtm_getRank...
-  Qed.
-
-  Local Hint Resolve subtm_asym : core.
-
-  Lemma subtm_trans :
-    forall M1 : tm,
-    forall M2 : tm,
-    forall M3 : tm,
-    subtm M1 M2 ->
-    subtm M2 M3 ->
-    subtm M1 M3.
-  Proof with eauto.
-    enough (claim1 : forall L : tm, forall N : tm, forall M : tm, subtm N L -> subtm M N -> subtm M L)...
-    induction L.
-    all: intros; inversion H; subst...
-    - constructor 2...
-    - constructor 3...
-    - constructor 4...
-  Qed.
-
-  Local Hint Resolve subtm_trans : core.
-
-  Theorem strong_induction_on_tm (phi : tm -> Prop) :
-    (forall M : tm, (forall N : tm, subtm N M -> N <> M -> phi N) -> phi M) ->
-    forall M : tm,
-    phi M.
-  Proof with try now (firstorder; eauto).
-    intros XXX.
-    enough (claim1 : forall M : tm, forall L : tm, subtm L M -> phi L)...
-    induction M.
-    all: intros L H; apply XXX; intros N H0 H1; inversion H0; subst...
-    all: inversion H; subst...
-  Qed.
-
-  Definition occurence_rect (XP : forall z : ivar, forall M : tm, subtm (tmVar z) M -> Type) :
-    (forall x : ivar, XP x (tmVar x) (subtmRefl (tmVar x))) ->
-    (forall x : ivar, forall P1 : tm, forall P2 : tm, forall X : subtm (tmVar x) P1, XP x P1 X -> XP x (tmApp P1 P2) (subtmAppL (tmVar x) P1 P2 X)) ->
-    (forall x : ivar, forall P1 : tm, forall P2 : tm, forall X : subtm (tmVar x) P2, XP x P2 X -> XP x (tmApp P1 P2) (subtmAppR (tmVar x) P1 P2 X)) ->
-    (forall x : ivar, forall y : ivar, forall Q : tm, forall X : subtm (tmVar x) Q, XP x Q X -> XP x (tmLam y Q) (subtmLAbs (tmVar x) y Q X)) ->
-    (forall x : ivar, forall M : tm, forall X : subtm (tmVar x) M, XP x M X).
-  Proof.
-    intros XP_refl XP_appl XP_appr XP_labs z.
-    assert ( XXX :
-      forall N : tm,
-      forall M : tm,
-      forall X : subtm N M,
-      forall H : N = tmVar z,
-      XP z M (eq_rect N (fun N0 : tm => subtm N0 M) X (tmVar z) H)
-    ).
-    { assert ( XP_Refl :
-        forall M0 : tm,
-        forall H : M0 = tmVar z,
-        XP z M0 (eq_rect M0 (fun N1 : tm => subtm N1 M0) (subtmRefl M0) (tmVar z) H)
-      ).
-      { intros M0.
-        apply (case_eq M0 (tmVar z) (fun M1 : tm => fun H0 : M1 = tmVar z => XP z M1 (eq_rect M1 (fun N1 : tm => subtm N1 M1) (subtmRefl M1) (tmVar z) H0))).
-        apply (XP_refl z).
-      }
-      assert ( XP_AppL :
-        forall M0 : tm,
-        forall P1 : tm,
-        forall P2 : tm,
-        forall H : M0 = tmVar z,
-        forall X' : subtm M0 P1,
-        (forall H' : M0 = tmVar z, XP z P1 (eq_rect M0 (fun N1 : tm => subtm N1 P1) X' (tmVar z) H')) ->
-        XP z (tmApp P1 P2) (eq_rect M0 (fun N1 : tm => subtm N1 (tmApp P1 P2)) (subtmAppL M0 P1 P2 X') (tmVar z) H)
-      ).
-      { intros M0 P1 P2.
-        apply (case_eq M0 (tmVar z) (fun M1 : tm => fun H0 : M1 = tmVar z => forall X' : subtm M1 P1, (forall H' : M1 = tmVar z, XP z P1 (eq_rect M1 (fun N1 : tm => subtm N1 P1) X' (tmVar z) H')) -> XP z (tmApp P1 P2) (eq_rect M1 (fun N1 : tm => subtm N1 (tmApp P1 P2)) (subtmAppL M1 P1 P2 X') (tmVar z) H0))).
-        apply (fun X' : subtm (tmVar z) P1 => fun IHX' : forall H' : tmVar z = tmVar z, XP z P1 (eq_rect (tmVar z) (fun N1 : tm => subtm N1 P1) X' (tmVar z) H') => XP_appl z P1 P2 X' (IHX' eq_refl)).
-      }
-      assert ( XP_AppR :
-        forall M0 : tm,
-        forall P1 : tm,
-        forall P2 : tm,
-        forall H : M0 = tmVar z,
-        forall X' : subtm M0 P2,
-        (forall H' : M0 = tmVar z, XP z P2 (eq_rect M0 (fun N1 : tm => subtm N1 P2) X' (tmVar z) H')) ->
-        XP z (tmApp P1 P2) (eq_rect M0 (fun N1 : tm => subtm N1 (tmApp P1 P2)) (subtmAppR M0 P1 P2 X') (tmVar z) H)
-      ).
-      { intros M0 P1 P2.
-        apply (case_eq M0 (tmVar z) (fun M1 : tm => fun H0 : M1 = tmVar z => forall X' : subtm M1 P2, (forall H' : M1 = tmVar z, XP z P2 (eq_rect M1 (fun N1 : tm => subtm N1 P2) X' (tmVar z) H')) -> XP z (tmApp P1 P2) (eq_rect M1 (fun N1 : tm => subtm N1 (tmApp P1 P2)) (subtmAppR M1 P1 P2 X') (tmVar z) H0))).
-        apply (fun X' : subtm (tmVar z) P2 => fun IHX' : forall H' : tmVar z = tmVar z, XP z P2 (eq_rect (tmVar z) (fun N1 : tm => subtm N1 P2) X' (tmVar z) H') => XP_appr z P1 P2 X' (IHX' eq_refl)).
-      }
-      assert ( XP_LAbs :
-        forall M0 : tm,
-        forall y : ivar,
-        forall Q : tm,
-        forall H : M0 = tmVar z,
-        forall X' : subtm M0 Q,
-        (forall H' : M0 = tmVar z, XP z Q (eq_rect M0 (fun N1 : tm => subtm N1 Q) X' (tmVar z) H')) ->
-        XP z (tmLam y Q) (eq_rect M0 (fun N1 : tm => subtm N1 (tmLam y Q)) (subtmLAbs M0 y Q X') (tmVar z) H)
-      ).
-      { intros M0 y Q.
-        apply (case_eq M0 (tmVar z) (fun M1 : tm => fun H0 : M1 = tmVar z => forall X' : subtm M1 Q, (forall H' : M1 = tmVar z, XP z Q (eq_rect M1 (fun N1 : tm => subtm N1 Q) X' (tmVar z) H')) -> XP z (tmLam y Q) (eq_rect M1 (fun N1 : tm => subtm N1 (tmLam y Q)) (subtmLAbs M1 y Q X') (tmVar z) H0))).
-        apply (fun X' : subtm (tmVar z) Q => fun IHX' : forall H' : tmVar z = tmVar z, XP z Q (eq_rect (tmVar z) (fun N1 : tm => subtm N1 Q) X' (tmVar z) H') => XP_labs z y Q X' (IHX' eq_refl)).
-      }
-      apply (
-        fix occurence_rect_fix (N : tm) (M : tm) (X : subtm N M) {struct X} : forall H : N = tmVar z, XP z M (eq_rect N (fun N1 : tm => subtm N1 M) X (tmVar z) H) :=
-        match X as X0 in subtm N0 M0 return forall H : N0 = tmVar z, XP z M0 (eq_rect N0 (fun N1 : tm => subtm N1 M0) X0 (tmVar z) H) with
-        | subtmRefl M0 =>
-          fun H : M0 = tmVar z =>
-          XP_Refl M0 H 
-        | subtmAppL M0 P1 P2 X' =>
-          fun H : M0 = tmVar z =>
-          XP_AppL M0 P1 P2 H X' (occurence_rect_fix M0 P1 X')
-        | subtmAppR M0 P1 P2 X' =>
-          fun H : M0 = tmVar z =>
-          XP_AppR M0 P1 P2 H X' (occurence_rect_fix M0 P2 X')
-        | subtmLAbs M0 y Q X' =>
-          fun H : M0 = tmVar z =>
-          XP_LAbs M0 y Q H X' (occurence_rect_fix M0 Q X')
-        end
-      ).
-    }
-    apply (
-      fun M : tm =>
-      fun X : subtm (tmVar z) M =>
-      XXX (tmVar z) M X eq_refl
-    ).
-  Defined.
-
-  Fixpoint getFVs (M : tm) : list ivar :=
-    match M with
-    | tmVar x => [x]
-    | tmApp P1 P2 => getFVs P1 ++ getFVs P2
-    | tmLam y Q => remove ivar_eq_dec y (getFVs Q)
-    end
-  .
-
-  Fixpoint isFreeIn (z : ivar) (M : tm) {struct M} : bool :=
-    match M with
-    | tmVar x => Nat.eqb x z
-    | tmApp P1 P2 => isFreeIn z P1 || isFreeIn z P2
-    | tmLam y Q => isFreeIn z Q && negb (Nat.eqb z y)
-    end
-  .
-
-  Lemma getFVs_isFreeIn (M : tm) :
-    forall z : ivar,
-    In z (getFVs M) <-> isFreeIn z M = true.
-  Proof with try now firstorder.
-    induction M; simpl; intros z.
-    - rewrite Nat.eqb_eq...
-    - rewrite orb_true_iff, in_app_iff...
-    - rewrite andb_true_iff, negb_true_iff, Nat.eqb_neq.
-      split; intros H.
-      + apply in_remove in H...
-      + apply in_in_remove...
-  Qed.
-
-  Definition substitution : Set :=
-    ivar -> tm
-  .
-
-  Definition nil_subtitution : substitution :=
-    tmVar
-  .
-
-  Definition cons_substitution : ivar -> tm -> substitution -> substitution :=
-    fun x : ivar => fun M : tm => fun sigma : substitution => fun y : ivar => if ivar_eq_dec x y then M else sigma y
-  .
-
-  Fixpoint mk_substitution (sigma : list (ivar * tm)) {struct sigma} : substitution :=
-    match sigma with
-    | [] => nil_subtitution
-    | (x, M) :: sigma' => cons_substitution x M (mk_substitution sigma')
-    end
-  .
-
-  Definition get_max_ivar : tm -> ivar :=
-    fun M : tm => fold_right_max_0 (getFVs M)
-  .
-
-  Lemma get_max_ivar_lt (M : tm) :
-    forall x : ivar,
-    get_max_ivar M < x ->
-    isFreeIn x M = false.
-  Proof with lia.
-    intros x.
-    enough (get_max_ivar M < x -> ~ In x (getFVs M)) by now rewrite getFVs_isFreeIn, not_true_iff_false in H.
-    assert (H1 : In x (getFVs M) -> fold_right_max_0 (getFVs M) >= x) by apply fold_right_max_0_in.
-    enough (fold_right_max_0 (getFVs M) >= x -> fold_right_max_0 (getFVs M) < x -> False) by now eauto...
-  Qed.
-
-  Definition isFreshIn_substitution : ivar -> substitution -> tm -> bool :=
-    fun x : ivar => fun sigma : substitution => fun M : tm => forallb (fun z : ivar => negb (isFreeIn x (sigma z))) (getFVs M)
-  .
-
-  Definition chi : substitution -> tm -> ivar :=
-    fun sigma : substitution => fun M : tm => S (fold_right_max_0 (map (fun x : ivar => get_max_ivar (sigma x)) (getFVs M)))
-  .
-
-  Theorem main_property_of_chi :
-    forall M : tm,
-    forall sigma : substitution,
-    isFreshIn_substitution (chi sigma M) sigma M = true.
-  Proof with try now firstorder.
-    assert ( claim1 :
-      forall sigma : substitution,
-      forall M : tm,
-      forall x : ivar,
-      isFreeIn x M = true ->
-      isFreeIn (chi sigma M) (sigma x) = false
-    ).
-    { intros sigma M x H.
-      enough (get_max_ivar (sigma x) < chi sigma M) by now apply get_max_ivar_lt.
-      unfold chi, fold_right_max_0.
-      enough (fold_right max 0 (map (fun z : ivar => get_max_ivar (sigma z)) (getFVs M)) >= get_max_ivar (sigma x)) by lia.
-      rewrite <- getFVs_isFreeIn in H.
-      apply fold_right_max_0_in, in_map_iff...
-    }
-    unfold isFreshIn_substitution.
-    intros M sigma.
-    apply forallb_true_iff.
-    intros x H.
-    apply negb_true_iff, claim1, getFVs_isFreeIn...
-  Qed.
-
-  Lemma chi_nil : 
-    forall M : tm,
-    isFreeIn (chi nil_subtitution M) M = false.
-  Proof with try now firstorder.
-    intros M.
-    assert (H : isFreshIn_substitution (chi nil_subtitution M) nil_subtitution M = true) by apply main_property_of_chi.
-    unfold isFreshIn_substitution in H.
-    rewrite forallb_true_iff in H.
-    simpl in H.
-    apply not_true_iff_false.
-    intros H0.
-    assert (H1 : negb (chi nil_subtitution M =? chi nil_subtitution M) = true) by now apply H, getFVs_isFreeIn.
-    rewrite negb_true_iff, Nat.eqb_neq in H1...
-  Qed.
-
-  Fixpoint run_substitution_on_tm (sigma : substitution) (M : tm) {struct M} : tm :=
-    match M with
-    | tmVar x => sigma x
-    | tmApp P1 P2 => tmApp (run_substitution_on_tm sigma P1) (run_substitution_on_tm sigma P2)
-    | tmLam y Q =>
-      let z : ivar := chi sigma M in
-      tmLam z (run_substitution_on_tm (cons_substitution y (tmVar z) sigma) Q)
-    end
-  .
-
-  Theorem main_property_isFreshIn_substitution :
-    forall M : tm,
-    forall z : ivar,
-    forall sigma : substitution,
-    isFreshIn_substitution z sigma M = true <-> isFreeIn z (run_substitution_on_tm sigma M) = false.
-  Proof with try now firstorder.
-    induction M; simpl.
-    - intros z sigma.
-      unfold isFreshIn_substitution.
-      simpl.
-      rewrite andb_true_iff, negb_true_iff...
-    - intros z sigma.
-      rewrite orb_false_iff.
-      unfold isFreshIn_substitution.
-      simpl.
-      rewrite forallb_app, andb_true_iff...
-    - intros z sigma.
-      rewrite andb_false_iff, negb_false_iff, Nat.eqb_eq.
-      unfold isFreshIn_substitution.
-      simpl.
-      rewrite forallb_true_iff.
-      split; intros H.
-      + destruct (ivar_eq_dec z (chi sigma (tmLam y M)))...
-        left.
-        apply IHM.
-        unfold isFreshIn_substitution.
-        rewrite forallb_true_iff.
-        intros x H0.
-        unfold cons_substitution.
-        destruct (ivar_eq_dec y x).
-        * unfold isFreeIn.
-          apply negb_true_iff, Nat.eqb_neq...
-        * apply H, in_in_remove...
-      + intros x H0.
-        apply in_remove in H0.
-        destruct H0.
-        destruct H.
-        * assert (H2 : isFreshIn_substitution z (cons_substitution y (tmVar (chi sigma (tmLam y M))) sigma) M = true) by now apply IHM.
-          unfold isFreshIn_substitution in H2.
-          rewrite forallb_true_iff in H2.
-          assert (H3 := H2 x H0).
-          unfold cons_substitution in H3.
-          destruct (ivar_eq_dec y x)...
-        * assert (H2 : isFreshIn_substitution z sigma (tmLam y M) = true).
-          { rewrite H.
-            apply main_property_of_chi...
-          }
-          unfold isFreshIn_substitution in H2.
-          rewrite forallb_true_iff in H2.
-          apply H2.
-          rewrite getFVs_isFreeIn.
-          simpl.
-          rewrite andb_true_iff, negb_true_iff, Nat.eqb_neq, <- getFVs_isFreeIn...
-  Qed.
-
-  Definition equiv_substitution_wrt : substitution -> substitution -> tm -> Prop :=
-    fun sigma1 : substitution => fun sigma2 : substitution => fun M : tm => forall x : ivar, isFreeIn x M = true -> sigma1 x = sigma2 x
-  .
-
-  Lemma property1_of_equiv_substitution_wrt :
-    forall sigma1 : substitution,
-    forall sigma2 : substitution,
-    (forall x : ivar, sigma1 x = sigma2 x) ->
-    forall M : tm,
-    equiv_substitution_wrt sigma1 sigma2 M.
-  Proof with try now firstorder.
-    unfold equiv_substitution_wrt...
-  Qed.
-
-  Lemma chi_equiv_substitution_wrt :
-    forall sigma1 : substitution,
-    forall sigma2 : substitution,
-    forall M : tm,
-    equiv_substitution_wrt sigma1 sigma2 M ->
-    chi sigma1 M = chi sigma2 M.
-  Proof with reflexivity.
-    unfold chi.
-    intros sigma1 sigma2 M H.
-    enough (H0 : (map (fun x : ivar => get_max_ivar (sigma1 x)) (getFVs M)) = (map (fun x : ivar => get_max_ivar (sigma2 x)) (getFVs M))) by congruence.
-    apply map_ext_in.
-    intros x H0.
-    rewrite (H x (proj1 (getFVs_isFreeIn M x) H0))...
-  Qed.
-
-  Theorem main_property_of_equiv_substitution_wrt :
-    forall M : tm,
-    forall sigma1 : substitution,
-    forall sigma2 : substitution,
-    equiv_substitution_wrt sigma1 sigma2 M ->
-    run_substitution_on_tm sigma1 M = run_substitution_on_tm sigma2 M.
-  Proof with try now firstorder.
-    induction M.
-    - intros sigma1 sigma2 H.
-      apply H.
-      simpl.
-      rewrite Nat.eqb_eq...
-    - intros sigma1 sigma2 H.
-      assert (H1 : equiv_substitution_wrt sigma1 sigma2 M1).
-      { intros x H0.
-        apply H.
-        simpl.
-        rewrite orb_true_iff...
-      }
-      assert (H2 : equiv_substitution_wrt sigma1 sigma2 M2).
-      { intros x H0.
-        apply H.
-        simpl.
-        rewrite orb_true_iff...
-      }
-      simpl.
-      rewrite (IHM1 sigma1 sigma2 H1), (IHM2 sigma1 sigma2 H2)...
-    - intros sigma1 sigma2 H.
-      simpl.
-      assert (H0 : equiv_substitution_wrt (cons_substitution y (tmVar (chi sigma1 (tmLam y M))) sigma1) (cons_substitution y (tmVar (chi sigma2 (tmLam y M))) sigma2) M).
-      { intros x H0.
-        unfold cons_substitution.
-        destruct (ivar_eq_dec y x).
-        - rewrite (chi_equiv_substitution_wrt sigma1 sigma2 (tmLam y M) H)...
-        - apply H.
-          simpl.
-          rewrite andb_true_iff, negb_true_iff, Nat.eqb_neq...
-      }
-      assert (H1 : chi sigma1 (tmLam y M) = chi sigma2 (tmLam y M)) by now apply chi_equiv_substitution_wrt.
-      rewrite (IHM (cons_substitution y (tmVar (chi sigma1 (tmLam y M))) sigma1) (cons_substitution y (tmVar (chi sigma2 (tmLam y M))) sigma2) H0), H1...
-  Qed.
-
-  Lemma trivial_substitution :
-    forall x : ivar,
-    forall M : tm,
-    run_substitution_on_tm (cons_substitution x (tmVar x) nil_subtitution) M = run_substitution_on_tm nil_subtitution M.
-  Proof with try now firstorder.
-    unfold cons_substitution.
-    intros x M.
-    apply main_property_of_equiv_substitution_wrt.
-    intros y H.
-    destruct (ivar_eq_dec x y)...
-  Qed.
-
-  Definition compose_substitution : substitution -> substitution -> substitution :=
-    fun sigma1 : substitution => fun sigma2 : substitution => fun x : ivar => run_substitution_on_tm sigma1 (sigma2 x)
-  .
-
-  Lemma distri_compose_cons :
-    forall M : tm,
-    forall N : tm,
-    forall sigma1 : substitution,
-    forall sigma2 : substitution,
-    forall x : ivar,
-    forall y : ivar,
-    isFreshIn_substitution y sigma1 (tmLam x M) = true ->
-    forall z : ivar,
-    isFreeIn z M = true ->
-    cons_substitution x N (compose_substitution sigma2 sigma1) z = compose_substitution (cons_substitution y N sigma2) (cons_substitution x (tmVar y) sigma1) z.
-  Proof with try now firstorder.
-    intros M N sigma1 sigma2 x y H z H0.
-    unfold cons_substitution, compose_substitution.
-    destruct (ivar_eq_dec x z).
-    - simpl.
-      destruct (ivar_eq_dec y y)...
-    - unfold isFreshIn_substitution in H.
-      rewrite forallb_true_iff in H.
-      assert (H1 : isFreeIn y (sigma1 z) = false).
-      { apply negb_true_iff, H, getFVs_isFreeIn.
-        simpl.
-        rewrite andb_true_iff, negb_true_iff, Nat.eqb_neq...
-      }
-      assert ( claim1 :
-        forall u : ivar,
-        isFreeIn u (sigma1 z) = true ->
-        cons_substitution y N sigma2 u = sigma2 u
-      ).
-      { unfold cons_substitution.
-        intros u H2.
-        destruct (ivar_eq_dec y u)...
-        subst.
-        rewrite H1 in H2...
-      }
-      apply main_property_of_equiv_substitution_wrt...
-  Qed.
-
-  Corollary distri_compose_cons_for_chi :
-    forall M : tm,
-    forall N : tm,
-    forall sigma1 : substitution,
-    forall sigma2 : substitution,
-    forall x : ivar,
-    let y : ivar := chi sigma1 (tmLam x M) in
-    forall z : ivar,
-    isFreeIn z M = true ->
-    cons_substitution x N (compose_substitution sigma2 sigma1) z = compose_substitution (cons_substitution y N sigma2) (cons_substitution x (tmVar y) sigma1) z.
-  Proof with eauto using distri_compose_cons, main_property_of_chi.
-    intros M N sigma1 sigma2 x y z H...
-  Qed.
-
-  Definition FreeIn_wrt : ivar -> substitution -> tm -> Prop :=
-    fun x : ivar => fun sigma : substitution => fun M : tm => exists y : ivar, isFreeIn y M = true /\ isFreeIn x (sigma y) = true
-  .
-
-  Theorem isFreeIn_wrt_true_iff (M : tm) :
-    forall z : ivar,
-    forall sigma : substitution,
-    isFreeIn z (run_substitution_on_tm sigma M) = true <-> FreeIn_wrt z sigma M.
-  Proof with try now firstorder.
-    unfold FreeIn_wrt.
-    induction M; simpl.
-    - intros z sigma.
-      split; intros H.
-      + exists x.
-        rewrite Nat.eqb_eq...
-      + destruct H as [y H].
-        rewrite Nat.eqb_eq in H.
-        destruct H.
-        subst...
-    - intros z sigma.
-      rewrite orb_true_iff.
-      split; intros H.
-      + destruct H; [enough (H0 : exists y : ivar, isFreeIn y M1 = true /\ isFreeIn z (sigma y) = true) | enough (H0 : exists y : ivar, isFreeIn y M2 = true /\ isFreeIn z (sigma y) = true)]...
-        all: destruct H0 as [y]; exists y; rewrite orb_true_iff...
-      + destruct H as [y].
-        rewrite orb_true_iff in H...
-    - intros x sigma.
-      rewrite andb_true_iff, negb_true_iff, Nat.eqb_neq.
-      split; intros H.
-      + destruct H.
-        assert (H1 := proj1 (IHM x (cons_substitution y (tmVar (chi sigma (tmLam y M))) sigma)) H).
-        destruct H1 as [w].
-        destruct H1.
-        set (z := chi sigma (tmLam y M)).
-        fold z in H, H0, H2.
-        destruct (ivar_eq_dec y w).
-        * subst.
-          unfold cons_substitution in H2.
-          destruct (ivar_eq_dec w w)...
-          unfold isFreeIn in H2.
-          rewrite Nat.eqb_eq in H2...
-        * exists w.
-          rewrite andb_true_iff, negb_true_iff, Nat.eqb_neq.
-          unfold cons_substitution in H2.
-          destruct (ivar_eq_dec y w)...
-      + rename y into z.
-        destruct H as [y].
-        destruct H.
-        set (w := chi sigma (tmLam z M)).
-        rewrite andb_true_iff, negb_true_iff, Nat.eqb_neq in H.
-        destruct (ivar_eq_dec w x).
-        * subst.
-          assert (isFreshIn_substitution w sigma (tmLam z M) = true) by now apply main_property_of_chi.
-          unfold isFreshIn_substitution in H1.
-          rewrite forallb_true_iff in H1.
-          enough (H2 : isFreeIn w (sigma y) = false) by now rewrite H0 in H2.
-          apply negb_true_iff, H1, getFVs_isFreeIn.
-          simpl.
-          rewrite andb_true_iff, negb_true_iff, Nat.eqb_neq...
-        * split...
-          apply IHM.
-          exists y.
-          split...
-          unfold cons_substitution.
-          destruct (ivar_eq_dec z y)...
-  Qed.
-
-  Lemma chi_ext :
-    forall sigma : substitution,
-    forall sigma' : substitution,
-    forall M : tm,
-    forall M' : tm,
-    (forall z : ivar, FreeIn_wrt z sigma M <-> FreeIn_wrt z sigma' M') ->
-    chi sigma M = chi sigma' M'.
-  Proof with try now firstorder.
-    unfold chi, FreeIn_wrt.
-    intros.
-    enough (fold_right_max_0 (map (fun x : ivar => get_max_ivar (sigma x)) (getFVs M)) = fold_right_max_0 (map (fun x : ivar => get_max_ivar (sigma' x)) (getFVs M'))) by lia.
-    assert ( claim1 :
-      forall z : ivar,
-      In z (flat_map (fun y : ivar => getFVs (sigma y)) (getFVs M)) <-> In z (flat_map (fun y : ivar => getFVs (sigma' y)) (getFVs M'))
-    ).
-    { intros z.
-      repeat (rewrite in_flat_map).
-      split; intros.
-      all: destruct H0 as [x]; rewrite getFVs_isFreeIn in H0.
-      1: assert (H1 : exists y : ivar, isFreeIn y M' = true /\ isFreeIn z (sigma' y) = true).
-      3: assert (H1 : exists y : ivar, isFreeIn y M = true /\ isFreeIn z (sigma y) = true).
-      1, 3: apply H; exists x...
-      1, 2: rewrite getFVs_isFreeIn in H0...
-      all: destruct H1 as [y]; exists y; repeat (rewrite getFVs_isFreeIn)...
-    }
-    assert (H0 : fold_right_max_0 (flat_map (fun y : ivar => getFVs (sigma y)) (getFVs M)) = fold_right_max_0 (flat_map (fun y : ivar => getFVs (sigma' y)) (getFVs M'))) by now apply fold_right_max_0_ext.
-    unfold get_max_ivar.
-    enough (H1 : forall xs : list ivar, forall f : ivar -> list ivar, fold_right_max_0 (map (fun x : ivar => fold_right_max_0 (f x)) xs) = fold_right_max_0 (flat_map f xs)) by now repeat (rewrite H1).
-    induction xs; simpl; intros f...
-    rewrite fold_right_max_0_app...
-  Qed.
-
-  Theorem main_property_of_compose_substitution :
-    forall M : tm,
-    forall sigma1 : substitution,
-    forall sigma2 : substitution,
-    run_substitution_on_tm sigma2 (run_substitution_on_tm sigma1 M) = run_substitution_on_tm (compose_substitution sigma2 sigma1) M.
-  Proof with try now firstorder.
-    induction M; simpl.
-    - intros sigma1 sigma2...
-    - intros sigma1 sigma2.
-      rewrite IHM1, IHM2...
-    - intros sigma1 sigma2.
-      enough (lemma : chi sigma2 (run_substitution_on_tm sigma1 (tmLam y M)) = chi (compose_substitution sigma2 sigma1) (tmLam y M)).
-      { set (x := chi sigma1 (tmLam y M)).
-        set (x' := chi sigma2 (tmLam x (run_substitution_on_tm (cons_substitution y (tmVar x) sigma1) M))).
-        set (z := chi (compose_substitution sigma2 sigma1) (tmLam y M)).
-        assert (H := IHM (cons_substitution y (tmVar x) sigma1) (cons_substitution x (tmVar x') sigma2)).
-        rewrite H.
-        assert (H0 : run_substitution_on_tm (compose_substitution (cons_substitution x (tmVar x') sigma2) (cons_substitution y (tmVar x) sigma1)) M = run_substitution_on_tm (cons_substitution y (tmVar x') (compose_substitution sigma2 sigma1)) M).
-        { apply main_property_of_equiv_substitution_wrt.
-          intros u H0.
-          assert (H1 := distri_compose_cons_for_chi M (tmVar x') sigma1 sigma2 y).
-          simpl in H1.
-          rewrite (H1 u H0)...
-        }
-        rewrite H0.
-        replace x' with z...
-      }
-      rename y into x.
-      set (y := chi sigma1 (tmLam x M)).
-      assert ( claim1 :
-        forall y' : ivar,
-        (exists x' : ivar, isFreeIn x' (tmLam y (run_substitution_on_tm (cons_substitution x (tmVar y) sigma1) M)) = true /\ isFreeIn y' (sigma2 x') = true) ->
-        (exists u : ivar, isFreeIn u (tmLam x M) = true /\ isFreeIn y' (compose_substitution sigma2 sigma1 u) = true)
-      ).
-      { intros y' H.
-        destruct H as [x'].
-        destruct H.
-        simpl in H.
-        rewrite andb_true_iff, negb_true_iff, Nat.eqb_neq in H.
-        destruct H.
-        assert (H2 := proj1 (isFreeIn_wrt_true_iff M x' (cons_substitution x (tmVar y) sigma1)) H).
-        destruct H2 as [u].
-        destruct H2.
-        unfold cons_substitution in H3.
-        destruct (ivar_eq_dec x u).
-        - unfold isFreeIn in H3.
-          rewrite Nat.eqb_eq in H3...
-        - exists u.
-          split.
-          + simpl.
-            rewrite andb_true_iff, negb_true_iff, Nat.eqb_neq...
-          + apply (proj2 (isFreeIn_wrt_true_iff (sigma1 u) y' sigma2))...
-      }
-      assert ( claim2 :
-        forall y' : ivar,
-        (exists x' : ivar, isFreeIn x' (tmLam x M) = true /\ isFreeIn y' (compose_substitution sigma2 sigma1 x') = true) ->
-        (exists u : ivar, isFreeIn u (tmLam y (run_substitution_on_tm (cons_substitution x (tmVar y) sigma1) M)) = true /\ isFreeIn y' (sigma2 u) = true)
-      ).
-      { intros y' H.
-        destruct H as [x'].
-        destruct H.
-        simpl in H.
-        rewrite andb_true_iff, negb_true_iff, Nat.eqb_neq in H.
-        destruct H.
-        assert (H2 := proj1 (isFreeIn_wrt_true_iff (sigma1 x') y' sigma2) H0).
-        destruct H2 as [u].
-        destruct H2.
-        assert (H4 : isFreeIn u (run_substitution_on_tm (cons_substitution x (tmVar y) sigma1) M) = true).
-        { apply isFreeIn_wrt_true_iff.
-          exists x'.
-          split...
-          unfold cons_substitution.
-          destruct (ivar_eq_dec x x')...
-        }
-        exists u.
-        split...
-        simpl.
-        rewrite andb_true_iff, negb_true_iff, Nat.eqb_neq.
-        split...
-        intros H5.
-        subst.
-        enough (H6 : isFreeIn y (sigma1 x') = false) by now rewrite H2 in H6.
-        assert (H5 := main_property_of_chi (tmLam x M) sigma1).
-        unfold isFreshIn_substitution in H5.
-        rewrite forallb_true_iff in H5.
-        apply negb_true_iff, H5.
-        rewrite getFVs_isFreeIn.
-        simpl.
-        rewrite andb_true_iff, negb_true_iff, Nat.eqb_neq...
-      }
-      apply chi_ext...
-  Qed.
-
-  Corollary compose_one :
-    forall M : tm,
-    forall N : tm,
-    forall sigma : substitution,
-    forall x : ivar,
-    run_substitution_on_tm (cons_substitution x (run_substitution_on_tm sigma N) sigma) M = run_substitution_on_tm sigma (run_substitution_on_tm (cons_substitution x N nil_subtitution) M).
-  Proof with try now firstorder.
-    intros M N sigma x.
-    replace (run_substitution_on_tm (cons_substitution x (run_substitution_on_tm sigma N) sigma) M) with (run_substitution_on_tm (cons_substitution x (run_substitution_on_tm sigma N) (compose_substitution sigma nil_subtitution)) M).
-    replace (run_substitution_on_tm (cons_substitution x (run_substitution_on_tm sigma N) (compose_substitution sigma nil_subtitution)) M) with (run_substitution_on_tm (compose_substitution sigma (cons_substitution x N nil_subtitution)) M).
-    rewrite main_property_of_compose_substitution...
-    all: apply main_property_of_equiv_substitution_wrt; apply property1_of_equiv_substitution_wrt; unfold compose_substitution, cons_substitution, nil_subtitution; intros z; destruct (ivar_eq_dec x z)...
-  Qed.
-
-  Theorem main_property_of_cons_substitution :
-    forall x : ivar,
-    forall z : ivar,
-    forall M : tm,
-    forall N : tm,
-    forall sigma : substitution,
-    isFreeIn z (tmLam x M) = false ->
-    run_substitution_on_tm (cons_substitution x N sigma) M = run_substitution_on_tm (cons_substitution z N sigma) (run_substitution_on_tm (cons_substitution x (tmVar z) nil_subtitution) M).
-  Proof with try now firstorder.
-    intros.
-    rewrite (main_property_of_compose_substitution M (cons_substitution x (tmVar z) nil_subtitution) (cons_substitution z N sigma)).
-    apply main_property_of_equiv_substitution_wrt.
-    intros w H0.
-    unfold cons_substitution, nil_subtitution, compose_substitution.
-    destruct (ivar_eq_dec x w); simpl.
-    - destruct (ivar_eq_dec z z)...
-    - destruct (ivar_eq_dec z w)...
-      simpl in H.
-      subst.
-      rewrite H0 in H.
-      simpl in H.
-      rewrite negb_false_iff, Nat.eqb_eq in H.
-      contradiction n...
-  Qed.
-
-  Class isPreLambdaStructure (D : Type) : Type :=
-    { runApp : D -> (D -> D)
-    ; runLam : (D -> D) -> D
-    }
-  .
-
-  Lemma runApp_ext {D : Type} `{D_isPreLambdaStructure : isPreLambdaStructure D} :
-    forall v1 : D,
-    forall v2 : D,
-    forall v1' : D,
-    forall v2' : D,
-    v1 = v1' ->
-    v2 = v2' ->
-    runApp v1 v2 = runApp v1' v2'.
-  Proof.
-    congruence.
-  Qed.
-
-  Global Hint Resolve runApp_ext : my_hints.
-
-  Lemma runLam_ext {D : Type} `{D_isPreLambdaStructure : isPreLambdaStructure D} :
-    forall vv : D -> D,
-    forall vv' : D -> D,
-    (forall v0 : D, vv v0 = vv' v0) ->
-    runLam vv = runLam vv'.
-  Proof.
-    intros vv vv' H.
-    apply functional_extensionality in H.
-    congruence.
-  Qed.
-
-  Global Hint Resolve runLam_ext : my_hints.
-
-  Definition eval_tm {D : Type} `{D_is_model : isPreLambdaStructure D} : (ivar -> D) -> tm -> D :=
-    fix eval_tm_fix (E : ivar -> D) (M : tm) {struct M} : D :=
-    match M with
-    | tmVar x => E x
-    | tmApp P1 P2 => runApp (eval_tm_fix E P1) (eval_tm_fix E P2)
-    | tmLam y Q => runLam (fun v : D => eval_tm_fix (fun z : ivar => if ivar_eq_dec y z then v else E z) Q)
-    end
-  .
-
-  Lemma eval_tm_ext {D : Type} `{D_is_model : isPreLambdaStructure D} :
-    forall M : tm,
-    forall E1 : ivar -> D,
-    forall E2 : ivar -> D,
-    (forall z : ivar, isFreeIn z M = true -> E1 z = E2 z) ->
-    eval_tm E1 M = eval_tm E2 M.
-  Proof with try now eauto with *.
-    induction M; simpl.
-    - intros E1 E2 H.
-      apply H.
-      rewrite Nat.eqb_eq...
-    - intros E1 E2 H.
-      rewrite (IHM1 E1 E2), (IHM2 E1 E2)...
-    - intros E1 E2 H.
-      enough (XXX : (fun v : D => eval_tm (fun z : ivar => if ivar_eq_dec y z then v else E1 z) M) = (fun v : D => eval_tm (fun z : ivar => if ivar_eq_dec y z then v else E2 z) M)) by congruence.
-      apply functional_extensionality.
-      intros v.
-      apply (IHM (fun z : ivar => if ivar_eq_dec y z then v else E1 z) (fun z : ivar => if ivar_eq_dec y z then v else E2 z))...
-      intros z H0.
-      destruct (ivar_eq_dec y z)...
-      apply H.
-      rewrite andb_true_iff, negb_true_iff, Nat.eqb_neq...
-  Qed.
-
-  Theorem run_substitution_on_tm_preserves_eval_tm {D : Type} `{D_is_model : isPreLambdaStructure D} :
-    forall M : tm,
-    forall sigma : substitution,
-    forall E : ivar -> D,
-    eval_tm (fun z : ivar => eval_tm E (sigma z)) M = eval_tm E (run_substitution_on_tm sigma M).
-  Proof with try now eauto with *.
-    induction M.
-    - intros sigma E...
-    - intros sigma E.
-      simpl...
-    - intros sigma E.
-      enough (claim1 : forall v : D, eval_tm (fun z : ivar => if ivar_eq_dec y z then v else eval_tm E (sigma z)) M = eval_tm (fun z : ivar => if ivar_eq_dec (chi sigma (tmLam y M)) z then v else E z) (run_substitution_on_tm (cons_substitution y (tmVar (chi sigma (tmLam y M))) sigma) M)) by now apply runLam_ext.
-      intros v.
-      assert (H := IHM (cons_substitution y (tmVar (chi sigma (tmLam y M))) sigma) (fun z : ivar => if ivar_eq_dec (chi sigma (tmLam y M)) z then v else E z)).
-      symmetry in H.
-      symmetry.
-      transitivity (eval_tm (fun z : ivar => eval_tm (fun z0 : ivar => if ivar_eq_dec (chi sigma (tmLam y M)) z0 then v else E z0) (cons_substitution y (tmVar (chi sigma (tmLam y M))) sigma z)) M)...
-      apply eval_tm_ext.
-      intros z H0.
-      unfold cons_substitution.
-      destruct (ivar_eq_dec y z).
-      + unfold eval_tm.
-        destruct (ivar_eq_dec (chi sigma (tmLam y M)) (chi sigma (tmLam y M)))...
-      + apply eval_tm_ext.
-        intros z' H1.
-        destruct (ivar_eq_dec (chi sigma (tmLam y M)) z')...
-        subst.
-        assert (H2 : isFreshIn_substitution (chi sigma (tmLam y M)) sigma (tmLam y M) = true) by now apply main_property_of_chi.
-        unfold isFreshIn_substitution in H2.
-        rewrite forallb_true_iff in H2.
-        enough (H3 : isFreeIn (chi sigma (tmLam y M)) (sigma z) = false) by now rewrite H3 in H1.
-        apply negb_true_iff, H2, getFVs_isFreeIn.
-        simpl.
-        rewrite andb_true_iff, negb_true_iff, Nat.eqb_neq...
-  Qed.
-
-End UntypedLamdbdaCalculus.
